wip

theories/Hoareproof1.v
@@ -30,6 +30,2338 @@ Set Implicit Arguments.
 
 
 
+Inductive _simg_safe (simg: forall R0 R1 (RR: R0 -> R1 -> Prop), Ord.t -> (itree eventE R0) -> (itree eventE R1) -> Prop)
+          {R0 R1} (RR: R0 -> R1 -> Prop) (i0: Ord.t): (itree eventE R0) -> (itree eventE R1) -> Prop :=
+| simg_safe_ret
+    r_src r_tgt
+    (SIM: RR r_src r_tgt)
+  :
+    _simg_safe simg RR i0 (Ret r_src) (Ret r_tgt)
+| simg_safe_syscall
+    i1 ktr_src0 ktr_tgt0 fn varg rvs
+    (SIM: forall x_src x_tgt (EQ: x_src = x_tgt), simg _ _ RR i1 (ktr_src0 x_src) (ktr_tgt0 x_tgt))
+  :
+    _simg_safe simg RR i0 (trigger (Syscall fn varg rvs) >>= ktr_src0) (trigger (Syscall fn varg rvs) >>= ktr_tgt0)
+
+
+
+| simg_safe_tau
+    i1 itr_src0 itr_tgt0
+    (TAUBOTH: True)
+    (* (ORD: Ordinal.le i1 i0) *)
+    (SIM: simg _ _ RR i1 itr_src0 itr_tgt0)
+  :
+    _simg_safe simg RR i0 (tau;; itr_src0) (tau;; itr_tgt0)
+| simg_safe_tauL
+    i1 itr_src0 itr_tgt0
+    (TAUL: True)
+    (ORD: Ord.lt i1 i0)
+    (SIM: simg _ _ RR i1 itr_src0 itr_tgt0)
+  :
+    _simg_safe simg RR i0 (tau;; itr_src0) (itr_tgt0)
+| simg_safe_tauR
+    i1 itr_src0 itr_tgt0
+    (TAUR: True)
+    (ORD: Ord.lt i1 i0)
+    (SIM: simg _ _ RR i1 itr_src0 itr_tgt0)
+  :
+    _simg_safe simg RR i0 (itr_src0) (tau;; itr_tgt0)
+
+
+
+| simg_safe_chooseR
+    i1 X itr_src0 ktr_tgt0
+    (CHOOSER: True)
+    (ORD: Ord.lt i1 i0)
+    (SIM: forall x, simg _ _ RR i1 itr_src0 (ktr_tgt0 x))
+  :
+    _simg_safe simg RR i0 (itr_src0) (trigger (Choose X) >>= ktr_tgt0)
+
+
+
+| simg_safe_takeL
+    i1 X ktr_src0 itr_tgt0
+    (TAKEL: True)
+    (ORD: Ord.lt i1 i0)
+    (SIM: forall x, simg _ _ RR i1 (ktr_src0 x) itr_tgt0)
+  :
+    _simg_safe simg RR i0 (trigger (Take X) >>= ktr_src0) (itr_tgt0)
+
+
+
+(* | simg_stutter *)
+(*     i1 itr_src itr_tgt *)
+(*     (ORD: Ord.lt i1 i0) *)
+(*     (SIM: simg _ RR i1 itr_src itr_tgt) *)
+(*   : *)
+(*     simg_safe simg RR i0 itr_src itr_tgt *)
+.
+
+Lemma simg_safe_spec:
+  _simg_safe <7= _simg.
+Proof. i. inv PR; try by (econs; eauto). Qed.
+
+
+
+
+
+
+
+
+
+
+
+
+
+
+
+
+
+
+(* Program Instance ord_lt_proper: Proper (Ord.eq ==> Ord.eq ==> eq) Ord.lt. *)
+(* Next Obligation. *)
+(*   ii. *)
+(*   apply prop_ext. split; i. *)
+(*   - eapply Ord.lt_eq_lt. { sym. et. } eapply Ord.eq_lt_lt; et. sym. et. *)
+(*   - eapply Ord.lt_eq_lt; et. eapply Ord.eq_lt_lt; et. *)
+(* Qed. *)
+
+Program Instance lt_proper: Proper (Ord.eq ==> Ord.eq ==> iff) (Ord.lt).
+Next Obligation.
+  ii.
+  split; i.
+  - eapply Ord.lt_eq_lt. { sym. et. } eapply Ord.eq_lt_lt; et. sym. et.
+  - eapply Ord.lt_eq_lt; et. eapply Ord.eq_lt_lt; et.
+Qed.
+
+Program Instance le_proper: Proper (Ord.eq ==> Ord.eq ==> iff) (Ord.le).
+Next Obligation.
+  ii.
+  split; i.
+  - eapply Ord.le_eq_le. { sym. et. } eapply Ord.eq_le_le; et. sym. et.
+  - eapply Ord.le_eq_le; et. eapply Ord.eq_le_le; et.
+Qed.
+
+Program Instance expn_proper: Proper (Ord.eq ==> Ord.eq ==> Ord.eq) (OrdArith.expn).
+Next Obligation.
+  ii.
+  etrans.
+  - eapply OrdArith.eq_expn_l; et.
+  - eapply OrdArith.eq_expn_r; et.
+Qed.
+
+Program Instance expn_le_proper: Proper (Ord.le ==> Ord.le ==> Ord.le) (OrdArith.expn).
+Next Obligation.
+  ii.
+  etrans.
+  - eapply OrdArith.le_expn_l; et.
+  - eapply OrdArith.le_expn_r; et.
+Qed.
+
+Program Instance add_proper: Proper (Ord.eq ==> Ord.eq ==> Ord.eq) (OrdArith.add).
+Next Obligation.
+  ii.
+  etrans.
+  - eapply OrdArith.eq_add_l; et.
+  - eapply OrdArith.eq_add_r; et.
+Qed.
+
+Program Instance add_le_proper: Proper (Ord.le ==> Ord.le ==> Ord.le) (OrdArith.add).
+Next Obligation.
+  ii.
+  etrans.
+  - eapply OrdArith.le_add_l; et.
+  - eapply OrdArith.le_add_r; et.
+Qed.
+
+(* Program Instance add_lt_proper: Proper (Ord.le ==> Ord.lt ==> Ord.lt) (OrdArith.add). *)
+(* Next Obligation. *)
+(*   ii. *)
+(*   eapply Ord.le_lt_lt. *)
+(*   - rewrite H. refl. *)
+(*   - eapply OrdArith.lt_add_r; et. *)
+(* Qed. *)
+
+Program Instance mult_eq_proper: Proper (Ord.eq ==> Ord.eq ==> Ord.eq) (OrdArith.mult).
+Next Obligation.
+  ii.
+  etrans.
+  - eapply OrdArith.eq_mult_l; et.
+  - eapply OrdArith.eq_mult_r; et.
+Qed.
+
+Program Instance mult_le_proper: Proper (Ord.le ==> Ord.le ==> Ord.le) (OrdArith.mult).
+Next Obligation.
+  ii.
+  etrans.
+  - eapply OrdArith.le_mult_l; et.
+  - eapply OrdArith.le_mult_r; et.
+Qed.
+
+Program Instance S_proper: Proper (Ord.eq ==> Ord.eq) (Ord.S).
+Next Obligation.
+  ii.
+  eapply Ord.eq_S; et.
+Qed.
+
+(* Program Instance eq_proper: Proper (Ord.eq ==> Ord.eq ==> Ord.eq) (Ord.lt). *)
+(* Next Obligation. *)
+(*   ii. *)
+(*   split; i. *)
+(*   - eapply Ord.lt_eq_lt. { sym. et. } eapply Ord.eq_lt_lt; et. sym. et. *)
+(*   - eapply Ord.lt_eq_lt; et. eapply Ord.eq_lt_lt; et. *)
+(* Qed. *)
+
+(* Theorem ord_pow_one: forall o0, (o0 ^ 1 == o0)%ord. *)
+(* Proof. *)
+(*   i. *)
+(*   unfold OrdArith.expn. *)
+(*   rewrite <- (OrdArith.add_O_r 1%ord). *)
+(*   rewrite OrdArith.expn_add. *)
+(*   replace (Ord.from_nat 1) with (1 + 0)%ord; cycle 1. *)
+(*   { rewrite OrdArith.add_O_r. Ord.add_0_r. *)
+(*   Set Printing All. *)
+(*   ss. *)
+(*   replace (1%ord) with (Ord.O + (1%ord))%ord. by ss. *)
+(*   etrans. rewrite OrdArith.expn_add. *)
+(* Qed. *)
+
+Lemma add_le_lt: forall x0 x1 y0 y1, (x0 <= x1)%ord -> (y0 < y1)%ord -> (x0 + y0 < x1 + y1)%ord.
+Proof.
+  i.
+  eapply Ord.le_lt_lt.
+  - eapply OrdArith.le_add_l; et.
+  - eapply OrdArith.lt_add_r; et.
+Qed.
+
+Lemma add_le_le: forall x0 x1 y0 y1, (x0 <= x1)%ord -> (y0 <= y1)%ord -> (x0 + y0 <= x1 + y1)%ord.
+Proof.
+  i.
+  etrans.
+  - eapply OrdArith.le_add_r; et.
+  - eapply OrdArith.le_add_l; et.
+Qed.
+
+Lemma mul_le_lt: forall x0 x1 y0 y1, (0 < x1)%ord -> (x0 <= x1)%ord -> (y0 < y1)%ord -> (x0 * y0 < x1 * y1)%ord.
+Proof.
+  i.
+  eapply Ord.le_lt_lt.
+  - eapply OrdArith.le_mult_l; et.
+  - eapply OrdArith.lt_mult_r; et.
+Qed.
+
+Lemma mult_le_le: forall x0 x1 y0 y1, (x0 <= x1)%ord -> (y0 <= y1)%ord -> (x0 * y0 <= x1 * y1)%ord.
+Proof.
+  i.
+  etrans.
+  - eapply OrdArith.le_mult_l; et.
+  - eapply OrdArith.le_mult_r; et.
+Qed.
+
+Lemma expn_pos: forall base o, (1 <= base ^ o)%ord.
+Proof. i. rewrite Ord.from_nat_S. eapply Ord.S_supremum. eapply OrdArith.expn_pos. Qed.
+
+Lemma add_one_lt: forall o0 o1, (o0 < o1)%ord -> (o0 + 1 <= o1)%ord.
+Proof.
+  i.
+  rewrite Ord.from_nat_S.
+  rewrite OrdArith.add_S.
+  rewrite OrdArith.add_O_r.
+  eapply Ord.S_supremum; et.
+Qed.
+
+
+
+
+
+
+Module Type PARAM.
+  Parameter c: Ord.t.
+  Parameter d: Ord.t.
+  Parameter e: Ord.t.
+  Parameter f: Ord.t.
+End PARAM.
+
+Module Construction (P: PARAM).
+  Include P.
+
+  Section CONSTRUCTION.
+
+  Let alpha := (f + 3 + d + e)%ord.
+  (* Let alpha_d: ((1 + d) <= alpha)%ord. *)
+  (* Proof. unfold alpha. rewrite <- OrdArith.add_O_r at 1. eapply add_le_le; try refl. eapply Ord.O_is_O. Qed. *)
+  Let alpha_e: (e <= alpha)%ord.
+  Proof.
+    unfold alpha.
+    eapply OrdArith.add_base_r.
+    (* etrans; [eapply OrdArith.add_base_l|]. *)
+    (* etrans; [eapply OrdArith.add_base_r|]. *)
+    (* rewrite <- OrdArith.add_assoc. rewrite OrdArith.add_assoc. refl. *)
+  Qed.
+
+  Let alpha_d: (f + 3 + d <= alpha)%ord.
+  Proof.
+    unfold alpha.
+    eapply OrdArith.add_base_l.
+    (* etrans; [eapply OrdArith.add_base_l|]. *)
+    (* etrans; [eapply OrdArith.add_base_r|]. *)
+    (* rewrite <- OrdArith.add_assoc. *)
+    (* eapply add_le_le; try refl. *)
+    (* rewrite <- OrdArith.add_assoc. *)
+    (* refl. *)
+  Qed.
+
+  Definition myF (o0: Ord.t): Ord.t := ((alpha * kappa + c) ^ (o0 + 1))%ord.
+  Definition myG (o0 m0: Ord.t): Ord.t := ((alpha * kappa + c) ^ (o0) * alpha * m0)%ord.
+  Definition myH (o0: Ord.t): Ord.t := ((alpha * kappa + c) ^ (o0) * 3)%ord.
+
+  (***
+                         (myG o0 kappa + d <= myF o0)
+  (AM: (m1 < m0)%ord) -> (myG o0 m1 + myH o0 + c <= myG o0 m0)%ord
+  (O: (o1 < o0)%ord)  -> (myF o1 + e <= myH o0)%ord
+   ***)
+
+  Let NZERO: (Ord.O < alpha * kappa + c)%ord.
+  Proof.
+    unfold alpha.
+
+    assert(T: (1 < f + 3 + d + e)%ord).
+    { assert(U: (1 + 1 <= (Ord.from_nat 3))%ord).
+      { rewrite <- OrdArith.add_from_nat. ss. eapply OrdArith.le_from_nat; et. }
+      eapply Ord.lt_le_lt; cycle 1.
+      { rewrite <- U. refl. }
+      rewrite ! OrdArith.add_assoc.
+      eapply Ord.lt_le_lt; cycle 1.
+      { eapply OrdArith.add_base_r. }
+      eapply OrdArith.add_lt_l.
+      rewrite Ord.from_nat_S at 1.
+      eapply Ord.lt_le_lt.
+      { instantiate (1:=1%ord). rewrite Ord.from_nat_S. eapply Ord.S_pos. }
+      { rewrite Ord.from_nat_S. eapply OrdArith.add_base_l. }
+    }
+
+    eapply Ord.lt_le_lt; cycle 1.
+    { eapply OrdArith.add_base_l. }
+    rewrite <- OrdArith.mult_1_r.
+    eapply Ord.le_lt_lt; cycle 1.
+    { instantiate (1:=((f + 3 + d + e) * 1)%ord).
+      eapply OrdArith.lt_mult_r.
+      - eauto with ord_kappa.
+      - rewrite <- T. replace (Ord.from_nat 1) with (Ord.S Ord.O) by ss. eapply Ord.S_pos. }
+    eapply mult_le_le.
+    - eapply Ord.O_is_O.
+    - refl.
+  Qed.
+
+  Global Program Instance myG_proper: Proper (Ord.le ==> Ord.le ==> Ord.le) (myG).
+  Next Obligation.
+    ii. unfold myG.
+    rewrite <- H0.
+    eapply mult_le_le; et; try refl.
+    eapply mult_le_le; et; try refl.
+    rewrite <- H. refl.
+  Qed.
+
+  Theorem my_thm1: forall o0, (myG o0 kappa + c <= myF o0)%ord.
+  Proof.
+    i. unfold myF, myG, myH.
+    rewrite OrdArith.expn_add; et.
+    rewrite OrdArith.expn_1_r; et.
+    rewrite OrdArith.mult_dist.
+    eapply add_le_le.
+    - rewrite <- OrdArith.mult_assoc. refl.
+    - rewrite <- (OrdArith.mult_1_l) at 1. eapply mult_le_le; try refl. eapply expn_pos.
+    (* OrdArith.add *)
+    (* OrdArith.mult *)
+    (* OrdArith.expn *)
+  Qed.
+
+  Theorem my_thm3
+          o0 o1
+          (O: (o1 < o0)%ord)
+    :
+      (myF o1 + e <= myH o0)%ord
+  .
+  Proof.
+    unfold myF, myG, myH.
+    eapply add_one_lt in O.
+    rewrite <- O.
+    rewrite OrdArith.expn_add; et.
+    rewrite OrdArith.expn_1_r; et.
+    assert(T: (1 + 1 <= 3)%ord).
+    { rewrite <- OrdArith.add_from_nat. ss. eapply OrdArith.le_from_nat; et. }
+    rewrite <- T.
+    rewrite OrdArith.mult_dist with (o2:=1).
+    rewrite OrdArith.mult_1_r.
+    eapply add_le_le; try refl.
+    rewrite <- (OrdArith.mult_1_l) at 1.
+    eapply mult_le_le.
+    { eapply expn_pos. }
+    rewrite <- alpha_e.
+    etrans; [|eapply OrdArith.add_base_l].
+    rewrite <- (OrdArith.mult_1_r) at 1.
+    eapply mult_le_le; try refl.
+    eapply Ord.lt_le.
+    eauto with ord_kappa.
+  Qed.
+
+  Theorem my_thm2
+          o0 m0 m1
+          (AM: (m1 < m0)%ord)
+    :
+      (myG o0 m1 + f + myH o0 + d <= myG o0 m0)%ord
+  .
+  Proof.
+    unfold myF, myG, myH.
+    eapply add_one_lt in AM.
+    rewrite <- AM.
+    rewrite OrdArith.mult_dist.
+    rewrite OrdArith.mult_1_r.
+    rewrite OrdArith.add_assoc.
+    rewrite OrdArith.add_assoc.
+    eapply add_le_le; try refl.
+    rewrite <- alpha_d at 3.
+    rewrite OrdArith.mult_dist.
+    rewrite OrdArith.mult_dist.
+    rewrite <- OrdArith.add_assoc.
+    eapply add_le_le; try refl; cycle 1.
+    { rewrite <- (OrdArith.mult_1_l) at 1. eapply mult_le_le; try refl. eapply expn_pos. }
+    eapply add_le_le; try refl; cycle 1.
+    { rewrite <- (OrdArith.mult_1_l) at 1. eapply mult_le_le; try refl. eapply expn_pos. }
+  Qed.
+
+  End CONSTRUCTION.
+
+End Construction.
+
+
+Module MyParam <: PARAM.
+  Definition d: Ord.t := 50%ord.
+  Definition c: Ord.t := (d + 30)%ord.
+  Definition e: Ord.t := 50%ord.
+  Definition f: Ord.t := (d + 10)%ord.
+End MyParam.
+
+Module C := (Construction MyParam).
+
+
+
+
+
+
+
+
+
+
+
+
+(* Lemma upcast_ty: forall T (v: T), Any.ty v↑ = T. admit "ez". Qed. *)
+(* Lemma upcast_val: forall T (v: T), Any.val v↑ ~= v. admit "ez". Qed. *)
+
+Lemma pair_downcast_lemma: forall T U (v0 v1: T) a (u: U), (Any.pair v0↑ a)↓ = Some (v1, u) -> v0 = v1 /\ a↓ = Some u.
+Proof.
+  admit "ez".
+Qed.
+
+
+
+
+
+
+Inductive opair: Type := mk_opair { ofst: Ord.t; osnd: Ord.t }.
+(* Definition opair_lt: opair -> opair -> Prop := fun '(mk_opair x0 x1) '(mk_opair y0 y1) => (x0 < y0)%ord \/ (x0 == y0 /\ x1 < y1)%ord. *)
+Inductive opair_lt: opair -> opair -> Prop :=
+| intro_opair_lt
+    x0 x1 y0 y1
+    (LT: (x0 < y0)%ord \/ (x0 == y0 /\ x1 < y1)%ord)
+  :
+    opair_lt (mk_opair x0 x1) (mk_opair y0 y1)
+.
+Theorem wf_opair_lt: well_founded opair_lt.
+Proof.
+  ii. destruct a.
+  revert osnd0. pattern ofst0. eapply well_founded_ind. { eapply Ord.lt_well_founded. } clear ofst0. intros ? IH0.
+  intro. generalize dependent x. pattern osnd0. eapply well_founded_ind. { eapply Ord.lt_well_founded. } clear osnd0. intros ? IH1.
+  econs. i. inv H. des.
+  { eapply IH0; et. }
+  { eapply IH1; et. i. eapply IH0; et. rewrite <- LT. ss. }
+Qed.
+
+
+
+
+
+
+
+
+
+
+
+Section CANCEL.
+
+  (*** execute following commands in emacs (by C-x C-e)
+     (progn (highlight-phrase "Any" 'hi-red-b) (highlight-phrase "Any_src" 'hi-green-b) (highlight-phrase "Any_tgt" 'hi-blue-b)
+            (highlight-phrase "Any_mid" 'hi-light-green-b)
+            (highlight-phrase "Y" 'hi-green-b) (highlight-phrase "Z" 'hi-green-b)) ***)
+  Let Any_src := Any.t. (*** src argument (e.g., List nat) ***)
+  Let Any_mid := Any.t. (*** src argument (e.g., List nat) ***)
+  Let Any_tgt := Any.t. (*** tgt argument (i.e., list val) ***)
+
+
+
+  Context `{Σ: GRA.t}.
+
+  Variable mds: list SMod.t.
+
+  Let sk: Sk.t := fold_right Sk.add Sk.unit (List.map SMod.sk mds).
+  (* Let skenv: SkEnv.t := Sk.load_skenv sk. *)
+  Let mss: list SModSem.t := (List.map ((flip SMod.get_modsem) sk) mds).
+  Let sbtb: list (gname * fspecbody) := (List.flat_map (SModSem.fnsems) mss).
+  Let stb: list (gname * fspec) := List.map (fun '(fn, fs) => (fn, fs.(fsb_fspec))) sbtb.
+
+  Let mds_src: list Mod.t := List.map (SMod.to_src) mds.
+  Let mds_mid: list Mod.t := List.map (SMod.to_mid stb) mds.
+
+
+
+  Let W: Type := (r_state * p_state).
+  (* Let wf: Ord.t -> W -> W -> Prop := top3. *)
+
+  Opaque EventsL.interp_Es.
+
+  Let ms_src: ModSemL.t := ModL.enclose (Mod.add_list mds_src).
+  Let ms_mid: ModSemL.t := ModL.enclose (Mod.add_list mds_mid).
+
+  Let p_src := ModSemL.prog ms_src.
+  Let p_mid := ModSemL.prog ms_mid.
+
+  Ltac _ord_step := eapply add_le_lt; [refl|eapply OrdArith.lt_from_nat; ss].
+
+  Ltac _step tac :=
+    match goal with
+    (*** terminal cases ***)
+    | [ |- gpaco6 _ _ _ _ _ _ _ _ (triggerUB >>= _) _ ] =>
+      unfold triggerUB; mred; _step tac; ss; fail
+    | [ |- gpaco6 _ _ _ _ _ _ _ _ (triggerNB >>= _) _ ] =>
+      exfalso
+    | [ |- gpaco6 _ _ _ _ _ _ _ _ _ (triggerUB >>= _) ] =>
+      exfalso
+    | [ |- gpaco6 _ _ _ _ _ _ _ _ _ (triggerNB >>= _) ] =>
+      unfold triggerNB; mred; _step tac; ss; fail
+
+    (*** assume/guarantee ***)
+    | [ |- gpaco6 _ _ _ _ _ _ _ _ (assume ?P ;;; _) _ ] =>
+      let tvar := fresh "tmp" in
+      let thyp := fresh "TMP" in
+      remember (assume P) as tvar eqn:thyp; unfold assume in thyp; subst tvar
+    | [ |- gpaco6 _ _ _ _ _ _ _ _ (guarantee ?P ;;; _) _ ] =>
+      let tvar := fresh "tmp" in
+      let thyp := fresh "TMP" in
+      remember (guarantee P) as tvar eqn:thyp; unfold guarantee in thyp; subst tvar
+    | [ |- gpaco6 _ _ _ _ _ _ _ _ _ (assume ?P ;;; _) ] =>
+      let tvar := fresh "tmp" in
+      let thyp := fresh "TMP" in
+      remember (assume P) as tvar eqn:thyp; unfold assume in thyp; subst tvar
+    | [ |- gpaco6 _ _ _ _ _ _ _ _ _ (guarantee ?P ;;; _) ] =>
+      let tvar := fresh "tmp" in
+      let thyp := fresh "TMP" in
+      remember (guarantee P) as tvar eqn:thyp; unfold guarantee in thyp; subst tvar
+
+    (*** default cases ***)
+    | _ =>
+      (gstep; tac; econs; auto; try (_ord_step);
+       (*** some post-processing ***)
+       i;
+       try match goal with
+           | [ |- (eq ==> _)%signature _ _ ] =>
+             let v_src := fresh "v_src" in
+             let v_tgt := fresh "v_tgt" in
+             intros v_src v_tgt ?; subst v_tgt
+           end)
+    end
+  .
+
+  Ltac steps := repeat (mred; try _step ltac:(eapply simg_safe_spec); des_ifs_safe).
+  Ltac steps_strong := repeat (mred; try (_step ltac:(idtac)); des_ifs_safe).
+
+  Lemma stb_find_iff fn
+    :
+      is_some (alist_find fn stb) <-> is_some (find (fun fnsem => dec fn (fst fnsem)) (fnsems ms_mid)).
+  Proof.
+    admit "in stb <-> in fnsems".
+  Qed.
+
+  Let adequacy_type_aux__APC:
+    forall at_most o0 mn
+           st_src0 st_tgt0
+    ,
+      simg (fun (st_src1: r_state * p_state * unit) '(st_tgt1, x) => st_tgt1 = st_tgt0)
+           (C.myG o0 at_most + C.d)%ord (Ret (st_src0, tt))
+           (EventsL.interp_Es p_mid (transl_all mn (interp_hCallE_mid stb (ord_pure o0) (_APC at_most))) st_tgt0)
+  .
+  Proof.
+    ginit.
+    { i. eapply cpn6_wcompat; eauto with paco. }
+    (* induction *)
+    intros ? ?. remember (mk_opair o0 at_most) as fuel. move fuel at top. revert at_most o0 Heqfuel.
+    pattern fuel. eapply well_founded_induction. { eapply wf_opair_lt. } clear fuel.
+    intros fuel IH. i.
+
+    rewrite unfold_APC. destruct st_tgt0 as [rst_tgt0 pst_tgt0]. steps.
+    destruct x.
+    { steps. }
+    steps. destruct (alist_find s stb) eqn:EQ; ss.
+    2: { steps. }
+    destruct rst_tgt0 as [mrs_tgt0 [|frs_hd frs_tl]]; ss.
+    { steps. destruct (Any.downcast t0); steps. }
+    steps. destruct (Any.downcast t0); ss.
+    2:{ steps. }
+    steps. unfold unwrapU. des_ifs; cycle 1.
+    { exfalso. hexploit (stb_find_iff s). rewrite EQ. rewrite Heq. clear. intuition. }
+    unfold ms_mid, mds_mid, SMod.to_mid in Heq. rewrite SMod.transl_fnsems in Heq.
+    unfold SMod.load_fnsems in Heq. apply find_some in Heq. des; ss. des_sumbool; subst.
+    rewrite in_flat_map in Heq. des; ss. rewrite in_flat_map in Heq0. des; ss. des_ifs. ss; des; ss; clarify.
+    rename Heq0 into INF. rename Heq into IN.
+    rename x3 into md0. fold sk in INF. fold sk in INF.
+    unfold fun_to_mid.
+    steps. assert (f0.(fsb_fspec) = f).
+    { admit "fspec table". }
+    subst. rewrite Any.upcast_downcast. steps.
+    guclo ordC_spec. econs.
+    { eapply OrdArith.add_base_l. }
+    guclo ordC_spec. econs.
+    { eapply C.my_thm2; et. }
+    guclo ordC_spec. econs.
+    { rewrite OrdArith.add_assoc. refl. }
+    rewrite idK_spec at 1.
+    guclo bindC_spec. econs.
+    { unfold APC. gstep. mred. eapply simg_chooseR; et; [_ord_step|]. i. steps.
+      guclo ordC_spec. econs.
+      { instantiate (1:=(C.myG x1 x3 + C.d)%ord).
+        rewrite <- C.my_thm3; et.
+        rewrite <- C.my_thm1; et.
+        rewrite OrdArith.add_assoc.
+        rewrite OrdArith.add_assoc.
+        eapply add_le_le.
+        - eapply Ord.lt_le in x4. rewrite <- x4. refl.
+        - etrans; [|eapply OrdArith.add_base_l]. etrans; [|eapply OrdArith.add_base_l]. refl.
+      }
+      eapply IH; auto. econs. left. auto.
+    }
+
+    i. ss. destruct vret_tgt as [? []]. destruct vret_src as [? []]. ss. des; subst.
+    unfold idK. unfold C.f.
+    guclo ordC_spec. econs.
+    { rewrite <- OrdArith.add_assoc. refl. }
+    steps.
+    guclo ordC_spec. econs.
+    { eapply OrdArith.add_base_l. }
+    { eapply IH; et. econs; et. right; split; et. refl. }
+  Qed.
+
+  Let adequacy_type_aux_APC:
+    forall o0 st_src0 st_tgt0 mn
+    ,
+      simg (fun (st_src1: r_state * p_state * unit) '(st_tgt1, _) => st_tgt1 = st_tgt0)
+           (C.myF o0)%ord (Ret (st_src0, tt))
+           (EventsL.interp_Es p_mid (transl_all mn (interp_hCallE_mid stb (ord_pure o0) APC)) st_tgt0)
+  .
+  Proof.
+    ginit.
+    { i. eapply cpn6_wcompat; eauto with paco. }
+    i. unfold APC.
+    guclo ordC_spec. econs.
+    { rewrite <- C.my_thm1. refl. }
+    unfold C.c.
+    guclo ordC_spec. econs.
+    { rewrite <- OrdArith.add_assoc. refl. }
+    steps.
+    guclo ordC_spec. econs.
+    { etrans; [|eapply OrdArith.add_base_l]. eapply add_le_le; [|refl].
+      instantiate (1:=C.myG o0 x).
+      eapply Ord.lt_le in x0. rewrite <- x0. refl. }
+    gfinal. right.
+    eapply adequacy_type_aux__APC.
+  Qed.
+
+  Lemma idK_spec2: forall E A B (a: A) (itr: itree E B), itr = Ret a >>= fun _ => itr. Proof. { i. ired. ss. } Qed.
+
+  Definition formula (o0: ord): Ord.t :=
+    match o0 with
+    | ord_pure o0 => (10 + C.myF o0)%ord
+    | ord_top => 100%ord
+    end
+  .
+
+  Let wf: W -> W -> Prop := fun '(_, pst_src0) '(_, pst_tgt0) => pst_src0 = pst_tgt0.
+  Let wf': forall {X}, (W * X)%type -> (W * X)%type -> Prop := (fun _ '(st_src0, rv_src) '(st_tgt0, rv_tgt) => wf st_src0 st_tgt0 /\ rv_src = rv_tgt).
+
+  Ltac resub :=
+    repeat multimatch goal with
+           | |- context[ITree.trigger ?e] =>
+             match e with
+             | subevent _ _ => idtac
+             | _ => replace (ITree.trigger e) with (trigger e) by refl
+             end
+           | |- context[@subevent _ ?F ?prf _ (?e|)%sum] => replace (@subevent _ F prf _ (e|)%sum) with (@subevent _ F _ _ e) by refl
+           | |- context[@subevent _ ?F ?prf _ (|?e)%sum] => replace (@subevent _ F prf _ (|e)%sum) with (@subevent _ F _ _ e) by refl
+           end.
+
+  Let adequacy_type_aux:
+    forall
+      o0
+      A (body: itree _ A) st_src0 st_tgt0 mn
+      (SIM: wf st_src0 st_tgt0)
+    ,
+      simg wf'
+           (formula o0 + 50)%ord
+           (EventsL.interp_Es p_src (transl_all mn (interp_hCallE_src body)) st_src0)
+           (EventsL.interp_Es p_mid (transl_all mn (interp_hCallE_mid stb o0 body)) st_tgt0)
+  .
+  Proof.
+    ginit.
+    { i. eapply cpn6_wcompat; eauto with paco. }
+    gcofix CIH. i. ides body.
+    { steps. }
+    { steps. gbase. eapply CIH; ss. }
+
+    destruct e; cycle 1.
+    { rewrite <- bind_trigger. resub. steps.
+      destruct s; ss.
+      { destruct st_src0 as [rst_src0 pst_src0]; ss. destruct st_tgt0 as [rst_tgt0 pst_tgt0]; ss.
+        destruct p; ss.
+        - steps. gbase. eapply CIH; ss; et.
+        - steps. gbase. eapply CIH; ss; et.
+      }
+      { dependent destruction e.
+        - steps_strong. exists x_tgt. steps. gbase. eapply CIH; et.
+        - steps_strong. exists x_src. steps. gbase. eapply CIH; et.
+        - steps_strong. gbase. eapply CIH; et.
+      }
+    }
+    dependent destruction h.
+    rewrite <- bind_trigger. resub.
+    destruct st_src0 as [rst_src0 pst_src0]; ss. destruct st_tgt0 as [rst_tgt0 pst_tgt0]; ss.
+    ired_both. destruct tbr.
+    (*
+PURE *)
+    { seal_left. steps. destruct (alist_find fn stb) eqn:EQ.
+      2: { steps. }
+      steps. destruct (Any.downcast varg_src).
+      2: { steps. }
+      Local Opaque ord_lt. steps.
+      destruct rst_tgt0 as [mrs_tgt0 [|frs_tgt_hd frs_tgt_tl]]; ss.
+      { steps. }
+      unseal_left. steps.
+      unfold unwrapU. des_ifs; cycle 1.
+      { exfalso. hexploit (stb_find_iff fn). rewrite EQ. rewrite Heq. clear. intuition. }
+      steps.
+
+      unfold ms_mid, mds_mid, SMod.to_mid in Heq. rewrite SMod.transl_fnsems in Heq.
+      unfold SMod.load_fnsems in Heq. apply find_some in Heq. des; ss. des_sumbool; subst.
+      rewrite in_flat_map in Heq. des; ss. rewrite in_flat_map in Heq0. des; ss. des_ifs. ss; des; ss; clarify.
+      rename Heq0 into INF. rename Heq into IN.
+      rename x0 into md0. fold sk in INF. fold sk in INF.
+      unfold fun_to_mid. ss.
+      assert (f = f0).
+      { admit "uniqueness". }
+      subst. rewrite Any.upcast_downcast. steps.
+      guclo ordC_spec. econs.
+      { eapply OrdArith.add_base_l. }
+
+      rewrite idK_spec2 at 1.
+      guclo bindC_spec. econs.
+      { gfinal. right. eapply paco6_mon. { eapply adequacy_type_aux_APC. } ii; ss. }
+      i. steps. steps_strong. exists (Any.upcast x0). steps.
+      gbase. eapply CIH. ss.
+    }
+
+    (* IMPURE *)
+    { seal_left. steps. destruct (alist_find fn stb) eqn:EQ.
+      2: { steps. }
+      steps. destruct (Any.downcast varg_src).
+      2: { steps. }
+      Local Opaque ord_lt. steps.
+      destruct rst_tgt0 as [mrs_tgt0 [|frs_tgt_hd frs_tgt_tl]]; ss.
+      { steps. }
+      unseal_left. steps.
+      unfold unwrapU. des_ifs; cycle 1.
+      { exfalso. hexploit (stb_find_iff fn). rewrite EQ. rewrite Heq. clear. intuition. }
+      steps.
+
+      unfold ms_mid, mds_mid, SMod.to_mid in Heq. rewrite SMod.transl_fnsems in Heq.
+      unfold SMod.load_fnsems in Heq. apply find_some in Heq. des; ss. des_sumbool; subst.
+      rewrite in_flat_map in Heq. des; ss. rewrite in_flat_map in Heq0. des; ss. des_ifs. ss; des; ss; clarify.
+      rename Heq0 into INF. rename Heq into IN.
+      rename x0 into md0. fold sk in INF. fold sk in INF.
+      unfold fun_to_mid. ss.
+      assert (f = f0).
+      { admit "uniqueness". }
+      subst. rewrite Any.upcast_downcast. steps.
+      guclo ordC_spec. econs.
+      { eapply OrdArith.add_base_l. }
+
+      rewrite idK_spec2 at 1.
+      guclo bindC_spec. econs.
+      { gfinal. right. eapply paco6_mon. { eapply adequacy_type_aux_APC. } ii; ss. }
+      i. steps. steps_strong. exists (Any.upcast x0). steps.
+      gbase. eapply CIH. ss.
+    }
+
+
+    }
+      { eapply OrdArith.add_base_l. instantiate (2:=formula o0). instantiate (1:=(100+C.myF x)%ord).
+        eapply OrdArith.add_base_l.
+
+
+        refl.
+
+
+      { instantiate (1:=_ + _). admit "". }
+      rewrite idK_spec2 at 1.
+      guclo bindC_spec. econs.
+      { gfinal. right. eapply paco6_mon. { eapply adequacy_type_aux_APC. } ii; ss. }
+      i. steps. steps_strong. exists (Any.upcast x0). steps.
+      gbase. eapply CIH. ss.
+    }
+
+      econs.
+      specialize (CIH0 o0 _ (k (Any.upcast x0)) (rst_src0, pst_tgt0) (mrs_tgt0, frs_tgt_hd :: frs_tgt_tl, pst_tgt0)).
+      instantiate (1:=Any.upcast x0).
+
+
+      eapply CIH0.
+
+      n
+
+      eapply adequacy_type_aux_APC.
+
+
+        unfold ms_mid, mds_mid, SMod.to_mid in Heq. rewrite SMod.transl_fnsems in Heq.
+        unfold SMod.load_fnsems in Heq. apply find_some in Heq. des; ss. des_sumbool; subst.
+        rewrite in_flat_map in Heq. des; ss. rewrite in_flat_map in Heq0. des; ss. des_ifs. ss; des; ss; clarify.
+        rename Heq0 into INF. rename Heq into IN.
+        rename x0 into md0. fold sk in INF. fold sk in INF.
+
+        unfold ms_src, mds_src, SMod.to_src in Heq0. rewrite SMod.transl_fnsems in Heq0.
+        unfold SMod.load_fnsems in Heq0. apply find_some in Heq0. des; ss. des_sumbool; subst.
+        rewrite in_flat_map in Heq0. des; ss. rewrite in_flat_map in Heq1. des; ss. des_ifs. ss; des; ss; clarify.
+        rename Heq1 into INF0. rename Heq0 into IN0.
+        rename x0 into md1. fold sk in INF0. fold sk in INF0.
+
+
+
+
+  Let adequacy_type_aux:
+    forall
+      AA AR
+      (args: AA)
+      o0
+      body st_src0 st_tgt0 mn
+      (SIM: wf st_src0 st_tgt0)
+    ,
+      simg wf'
+           (formula o0 + 10)%ord
+           (EventsL.interp_Es p_src (transl_all mn (if is_pure o0 then trigger (Choose _) else ((fun_to_src (AA:=AA) (AR:=AR) body) args↑))) st_src0)
+           (EventsL.interp_Es p_mid (transl_all mn ((fun_to_mid stb body) (o0, args)↑)) st_tgt0)
+  .
+  Proof.
+    ginit.
+    { i. eapply cpn6_wcompat; eauto with paco. }
+    gcofix CIH. i.
+    unfold fun_to_src, fun_to_mid. steps.
+    rewrite Any.upcast_downcast. steps.
+    unfold body_to_src, cfun. rewrite Any.upcast_downcast. ss. steps.
+    destruct o0; ss.
+    - (*** PURE ***)
+      seal_left.
+      steps.
+      unseal_left.
+      erewrite idK_spec2 at 1.
+      guclo ordC_spec. econs.
+      { eapply OrdArith.add_base_l. }
+      guclo bindC_spec.
+      econs.
+      { gfinal. right. eapply paco6_mon. { eapply adequacy_type_aux_APC. } ii; ss. }
+      ii; ss. des_ifs. des_u.
+      steps_strong. esplits; eauto. steps.
+    - (*** IMPURE ***)
+      steps. unfold body_to_mid.
+      abstr (body args) itr. clear body args AA.
+
+      guclo ordC_spec. econs.
+      { instantiate (1:=(10 + 100)%ord). rewrite <- ! OrdArith.add_from_nat. ss. refl. }
+      (* { instantiate (1:=(1 + 99)%ord). rewrite <- OrdArith.add_from_nat. ss. refl. } *)
+      guclo bindC_spec. eapply bindR_intro with (RR:=wf'); cycle 1.
+      { ii. subst. des_ifs. steps. r in SIM0. des; subst; ss. }
+
+      revert_until CIH. gcofix CIH0. i.
+
+      ides itr.
+      { steps. }
+      { steps. gbase. eapply CIH0; ss. }
+      destruct e; cycle 1.
+      {
+        rewrite <- bind_trigger. resub. steps.
+        destruct s; ss.
+        {
+          destruct st_src0 as [rst_src0 pst_src0]; ss. destruct st_tgt0 as [rst_tgt0 pst_tgt0]; ss.
+          destruct p; ss.
+          - steps. instantiate (1:=100). gbase. eapply CIH0; ss; et.
+          - steps. instantiate (1:=100). gbase. eapply CIH0; ss; et.
+        }
+        { dependent destruction e.
+          - steps_strong. unshelve esplits; et. instantiate (1:=100). steps. gbase. eapply CIH0; ss; et.
+          - steps_strong. unshelve esplits; et. instantiate (1:=100). steps. gbase. eapply CIH0; ss; et.
+          - steps_strong. unshelve esplits; et. instantiate (1:=100). steps. gbase. eapply CIH0; ss; et.
+        }
+      }
+      dependent destruction h.
+      rewrite <- bind_trigger. resub.
+      Opaque fun_to_src fun_to_mid.
+
+      destruct st_src0 as [rst_src0 pst_src0]; ss. destruct st_tgt0 as [rst_tgt0 pst_tgt0]; ss.
+      ired_both.
+      destruct tbr.
+      + (*** PURE CALL ***)
+        mred. steps.
+
+        (* seal_left. *)
+        (* Ltac step := (mred; try _step; des_ifs_safe). *)
+        (* step; try by eapply OrdArith.lt_from_nat. *)
+        (* step; try by eapply OrdArith.lt_from_nat. *)
+        (* unseal_left. *)
+        (* steps_strong. *)
+        (* set ((120 + formula (ord_pure x) + 100)%ord). *)
+        (* instantiate (1:=(120 + formula (ord_pure x) + 100)%ord). *)
+        (* seal_left. *)
+
+        destruct (alist_find fn stb) eqn:EQ.
+        2:{ steps. }
+        steps.
+        destruct (Any.downcast varg_src) eqn:ARG.
+        2:{ steps. }
+        steps.
+        destruct rst_tgt0 as [mrs_tgt0 [|frs_tgt_hd frs_tgt_tl]]; ss.
+        { steps. }
+        steps.
+        unfold unwrapU. des_ifs; cycle 1.
+        { admit "". }
+        steps_strong. eexists. steps.
+        unfold ms_mid, mds_mid, SMod.to_mid in Heq. rewrite SMod.transl_fnsems in Heq.
+        unfold SMod.load_fnsems in Heq. apply find_some in Heq. des; ss. des_sumbool; subst.
+        rewrite in_flat_map in Heq. des; ss. rewrite in_flat_map in Heq0. des; ss. des_ifs. ss; des; ss; clarify.
+        rename Heq0 into INF. rename Heq into IN.
+        rename x1 into md0. fold sk in INF. fold sk in INF.
+        mred.
+        guclo ordC_spec. econs.
+        {
+
+          admit "".
+          (* instantiate (1:=(120 + (10 + C.myF x + 10))%ord). *)
+          (* rewrite <- ! OrdArith.add_assoc. eapply add_le_le; try refl. eapply OrdArith.le_from_nat; ss. lia. *)
+
+        }
+        rename x into o1.
+        rewrite <- bind_bind.
+        rewrite <- bind_bind.
+        guclo bindC_spec. econs.
+        * (* guclo ordC_spec. econs. *)
+          (* { eapply OrdArith.add_base_r. } *)
+          (* gbase. eapply CIH; et. *)
+          gbase. hexploit CIH; et.
+          { instantiate (1:=(mrs_tgt0, ε :: frs_tgt_hd :: frs_tgt_tl, pst_tgt0)). instantiate (1:= (rst_src0, pst_tgt0)). ss. }
+          intro T. instantiate (2:=(ord_pure o1)) in T. ss.
+          mred.
+          (*** applying reduction in "T" begin ***)
+          (*** TODO: make prw "in" tactic ***)
+          revert T. pose (fun (x: Prop) (y: Prop) => (x -> y)) as myf.
+          match goal with | |- ?a -> ?b => replace (a -> b) with (myf a b) by refl end.
+          try Red.prw ltac:(IRed._red_gen) 2 2 0.
+          subst myf; cbn. intro T.
+          (*** applying reduction in "T" end ***)
+          eapply T.
+        * ii. des_ifs. destruct p, p0; ss. des; subst.
+          step; try by eapply OrdArith.lt_from_nat. steps.
+          destruct r1; ss.
+          des_ifs.
+          { unfold triggerNB. steps; try by eapply OrdArith.lt_from_nat. (*** TODO: fix tactic, don't unfold triggerNB ***) }
+          repeat (step; try by eapply OrdArith.lt_from_nat).
+          guclo ordC_spec. econs.
+          { instantiate (1:=100%ord). eapply OrdArith.le_from_nat; ss. lia. }
+          gbase. eapply CIH0. ss.
+      + (*** IMPURE CALL ***)
+        mred.
+        destruct rst_src0 as [mrs_src0 [|frs_src_hd frs_src_tl]]; ss.
+        { admit "SOMEHOW". }
+        mred. steps. instantiate (2:=(100 + (100 + 10) + 42)%ord). instantiate (1:=0%ord).
+        guclo ordC_spec. econs. { rewrite OrdArith.add_O_r. refl. }
+        destruct rst_tgt0 as [mrs_tgt0 [|frs_tgt_hd frs_tgt_tl]]; ss.
+        { steps. }
+        steps. unfold unwrapU at 2. des_ifs; cycle 1.
+        { admit "unwrapN!!!!!!!!!!!!!!!!!!". }
+        steps.
+        unfold unwrapU. des_ifs; cycle 1.
+        { steps. }
+        steps.
+
+        unfold ms_mid, mds_mid, SMod.to_mid in Heq. rewrite SMod.transl_fnsems in Heq.
+        unfold SMod.load_fnsems in Heq. apply find_some in Heq. des; ss. des_sumbool; subst.
+        rewrite in_flat_map in Heq. des; ss. rewrite in_flat_map in Heq1. des; ss. des_ifs. ss; des; ss; clarify.
+        rename Heq1 into INF. rename Heq into IN.
+        rename x0 into md0. fold sk in INF. fold sk in INF.
+
+        unfold ms_src, mds_src, SMod.to_src in Heq0. rewrite SMod.transl_fnsems in Heq0.
+        unfold SMod.load_fnsems in Heq0. apply find_some in Heq0. des; ss. des_sumbool; subst.
+        rewrite in_flat_map in Heq0. des; ss. rewrite in_flat_map in Heq1. des; ss. des_ifs. ss; des; ss; clarify.
+        rename Heq1 into INF0. rename Heq0 into IN0.
+        rename x0 into md1. fold sk in INF0. fold sk in INF0.
+
+        assert(md0 = md1); subst.
+        { admit "ez - uniqueness". }
+
+        assert(f = f0); subst.
+        { admit "ez - uniqueness". }
+
+        guclo ordC_spec. econs.
+        { eapply OrdArith.add_base_l. }
+        guclo bindC_spec.
+        econs.
+        * hexploit CIH; et; cycle 1.
+          { intro T. gbase. instantiate (3:=ord_top) in T. ss. eapply T. }
+          { ss. }
+        * ii; ss. des_ifs. steps. destruct p, p0; ss. des; subst.
+          steps. destruct r1; ss. des_ifs.
+          { unfold triggerNB. (step; try by eapply OrdArith.lt_from_nat). (*** TODO: fix tactic ***) }
+          destruct r0; ss. des_ifs. { admit "somehow". } steps.
+          instantiate (1:=100).
+          gbase. eapply CIH0 ;ss.
+  Unshelve.
+    all: try (by econs; et).
+    all: try (by exact Ord.O).
+    all: ss.
+  Unshelve.
+    all: try (by exact unit).
+  Qed.
+
+  Theorem adequacy_type_m2s: Beh.of_program (ModL.compile (Mod.add_list mds_mid)) <1=
+                             Beh.of_program (ModL.compile (Mod.add_list mds_src)).
+  Proof.
+    eapply adequacy_global.
+    exists (100)%ord. ss.
+    ginit.
+    { eapply cpn5_wcompat; eauto with paco. }
+    unfold ModSemL.initial_itr. Local Opaque ModSemL.prog. ss.
+    unfold ITree.map.
+    unfold assume.
+    steps.
+    instantiate (1:=(10 + (100 + 10) + 42)%ord).
+    esplits; et. { admit "ez - wf". } steps.
+    Local Transparent ModSemL.prog.
+    unfold ModSemL.prog at 4.
+    unfold ModSemL.prog at 2.
+    Local Opaque ModSemL.prog.
+    ss. steps.
+    (* Opaque ModSemL.initial_r_state. *)
+    (* Opaque ModSemL.initial_p_state. *)
+    fold ms_src. fold ms_mid.
+    set (rs_src0 := initial_r_state ms_src) in *.
+    set (rs_tgt0 := initial_r_state ms_mid) in *.
+    assert(exists mrs_src0 hd_src tl_src, rs_src0 = (mrs_src0, hd_src :: tl_src)).
+    { esplits. refl. }
+    assert(exists mrs_tgt0 hd_tgt tl_tgt, rs_tgt0 = (mrs_tgt0, hd_tgt :: tl_tgt)).
+    { esplits. refl. }
+    des. clearbody rs_src0 rs_tgt0. subst.
+    unfold unwrapU at 1. des_ifs; cycle 1.
+    { steps. }
+    unfold unwrapU. des_ifs; cycle 1.
+    { admit "unwrapN!!!!!!!!!!". }
+
+
+    unfold ms_mid, mds_mid, SMod.to_mid in Heq0. rewrite SMod.transl_fnsems in Heq0.
+    unfold SMod.load_fnsems in Heq0. apply find_some in Heq0. des; ss. des_sumbool; subst.
+    rewrite in_flat_map in Heq0. des; ss. rewrite in_flat_map in Heq2. des; ss. des_ifs. ss; des; ss; clarify. ss. subst.
+    rename Heq2 into INF. rename Heq0 into IN.
+    rename x into md0. fold sk in INF. fold sk in INF.
+
+    unfold ms_src, mds_src, SMod.to_src in Heq. rewrite SMod.transl_fnsems in Heq.
+    unfold SMod.load_fnsems in Heq. apply find_some in Heq. des; ss. destruct p; ss. des_sumbool; subst.
+    rewrite in_flat_map in Heq. des; ss. rewrite in_flat_map in Heq0. des; ss. des_ifs. ss; des; ss; clarify.
+    rename Heq0 into INF0. rename Heq into IN0.
+    rename x into md1. fold sk in INF0. fold sk in INF0.
+
+    assert(md0 = md1); subst.
+    { admit "ez - uniqueness". }
+    assert(f = f0).
+    { admit "ez - uniqueness". }
+    subst.
+    fold ms_src. fold ms_mid. fold p_src. fold p_mid.
+
+    steps.
+
+    match goal with
+    | [ |- gpaco5 _ _ _ _ _ _ _ ?i_src _ ] => remember i_src as tmp
+    end.
+    replace (([]: list val)↑) with (Any.pair ord_top↑ ([]: list val)↑) by admit "TODO".
+    subst tmp.
+
+    guclo ordC_spec. econs.
+    { eapply OrdArith.add_base_l. }
+    guclo bindC_spec.
+    econs.
+    - hexploit adequacy_type_aux; cycle 1.
+      { intro T. gfinal. right. instantiate (3:=ord_top) in T. ss. eapply T. }
+      ss. unfold ms_src, ms_mid. unfold initial_p_state.
+      apply func_ext. intro mn. unfold mds_src, mds_mid, SMod.to_src, SMod.to_mid.
+      rewrite ! SMod.transl_initial_mrs. ss.
+    - ii. rr in SIM. des_ifs. des; ss. subst. r in SIM. des_ifs. steps.
+  Unshelve.
+    all: ss.
+    all: try (by exact Ord.O).
+    all: try (by econs; et).
+  Qed.
+
+  (*** TODO: remove redundancy with Hoareproof0 ***)
+  Ltac resub :=
+    repeat multimatch goal with
+           | |- context[ITree.trigger ?e] =>
+             match e with
+             | subevent _ _ => idtac
+             | _ => replace (ITree.trigger e) with (trigger e) by refl
+             end
+           | |- context[@subevent _ ?F ?prf _ (?e|)%sum] => replace (@subevent _ F prf _ (e|)%sum) with (@subevent _ F _ _ e) by refl
+           | |- context[@subevent _ ?F ?prf _ (|?e)%sum] => replace (@subevent _ F prf _ (|e)%sum) with (@subevent _ F _ _ e) by refl
+           end.
+
+  Let adequacy_type_aux:
+    forall
+      o0
+      A (body: itree _ A) st_src0 st_tgt0 mn
+      (SIM: wf st_src0 st_tgt0)
+    ,
+      simg wf'
+           100%ord
+           (EventsL.interp_Es p_src (transl_all mn (interp_hCallE_src body)) st_src0)
+           (EventsL.interp_Es p_mid (transl_all mn (interp_hCallE_mid stb o0 body)) st_tgt0)
+  .
+  Proof.
+    ginit.
+    { i. eapply cpn5_wcompat; eauto with paco. }
+    gcofix CIH. i. ides body.
+    { steps. }
+    { steps. gbase. eapply CIH; ss. }
+
+    destruct e; cycle 1.
+    { rewrite <- bind_trigger. resub. steps.
+      destruct s; ss.
+      { destruct st_src0 as [rst_src0 pst_src0]; ss. destruct st_tgt0 as [rst_tgt0 pst_tgt0]; ss.
+        destruct p; ss.
+        - steps. gbase. eapply CIH; ss; et.
+        - steps. gbase. eapply CIH; ss; et.
+      }
+      { dependent destruction e.
+        - steps_strong. exists x_tgt. steps. gbase. eapply CIH; et.
+        - steps_strong. exists x_src. steps. gbase. eapply CIH; et.
+        - steps_strong. gbase. eapply CIH; et.
+      }
+    }
+    dependent destruction h.
+    rewrite <- bind_trigger. resub.
+    destruct st_src0 as [rst_src0 pst_src0]; ss. destruct st_tgt0 as [rst_tgt0 pst_tgt0]; ss.
+    ired_both. destruct tbr.
+    (* PURE *)
+    { steps_strong.
+      { admit "". }
+      eexists. steps. destruct (alist_find fn stb) eqn:EQ.
+      2: { steps. }
+      steps. destruct (Any.downcast varg_src).
+      2: { steps. }
+      steps. destruct rst_tgt0 as [mrs_tgt0 [|frs_tgt_hd frs_tgt_tl]]; ss.
+      { steps. }
+      steps. clear x0. unfold unwrapU. des_ifs; cycle 1.
+      { exfalso. hexploit (stb_find_iff fn). rewrite EQ. rewrite Heq. clear. intuition. }
+      steps.
+
+      guclo ordC_spec. econs.
+      { instantiate (1:=_ + _). admit "". }
+      rewrite idK_spec2 at 1.
+      guclo bindC_spec. econs.
+      {
+
+
+  Let adequacy_type_aux:
+    forall
+      AA AR
+      args
+      o0
+      body st_src0 st_tgt0 mn
+      (SIM: wf st_src0 st_tgt0)
+    ,
+      simg wf'
+           (formula o0 + 10)%ord
+           (* (if is_pure o0 then trigger (Choose _) else (interp_Es p_src ((fun_to_src (AA:=AA) (AR:=AR) body) args↑) st0)) *)
+           (EventsL.interp_Es p_src (transl_all mn (if is_pure o0 then trigger (Choose _) else ((fun_to_src (AA:=AA) (AR:=AR) body) args))) st_src0)
+           (EventsL.interp_Es p_mid (transl_all mn ((fun_to_mid stb body) (Any.pair o0↑ args))) st_tgt0)
+  .
+  Proof.
+    ginit.
+    { i. eapply cpn5_wcompat; eauto with paco. }
+    gcofix CIH. i.
+    unfold fun_to_src, fun_to_mid. steps. unfold unwrapN.
+    destruct (Any.downcast (Any.pair (Any.upcast o0) args)) eqn:T; cycle 1.
+    { steps. }
+    destruct p.
+    eapply pair_downcast_lemma in T. des; subst; ss. eapply Any.downcast_upcast in T0. des; subst.
+    unfold body_to_src, cfun. steps. rewrite Any.upcast_downcast. ss. steps.
+    destruct o; ss.
+    - (*** PURE ***)
+      seal_left.
+      steps.
+      unseal_left.
+      erewrite idK_spec2 at 1.
+      guclo ordC_spec. econs.
+      { eapply OrdArith.add_base_l. }
+      guclo bindC_spec.
+      econs.
+      { gfinal. right. eapply paco5_mon. { eapply adequacy_type_aux_APC. } ii; ss. }
+      ii; ss. des_ifs. des_u.
+      steps_strong. eexists. steps.
+    -
+
+      { admit "". }
+      esplits; eauto.
+
+      ste
+ steps.
+    - (*** IMPURE ***)
+      steps. unfold body_to_mid.
+      abstr (body a) itr. clear body a AA.
+
+      guclo ordC_spec. econs.
+      { instantiate (1:=(10 + 100)%ord). rewrite <- ! OrdArith.add_from_nat. ss. refl. }
+      (* { instantiate (1:=(1 + 99)%ord). rewrite <- OrdArith.add_from_nat. ss. refl. } *)
+      guclo bindC_spec. eapply bindR_intro with (RR:=wf'); cycle 1.
+      { ii. subst. des_ifs. steps. r in SIM0. des; subst; ss. }
+
+      revert_until CIH. gcofix CIH0. i.
+
+      ides itr.
+      { steps. }
+      { steps. gbase. eapply CIH0; ss. }
+      destruct e; cycle 1.
+      {
+
+        (*** TODO: remove redundancy with Hoareproof0 ***)
+  Ltac resub :=
+    repeat multimatch goal with
+           | |- context[ITree.trigger ?e] =>
+             match e with
+             | subevent _ _ => idtac
+             | _ => replace (ITree.trigger e) with (trigger e) by refl
+             end
+           | |- context[@subevent _ ?F ?prf _ (?e|)%sum] => replace (@subevent _ F prf _ (e|)%sum) with (@subevent _ F _ _ e) by refl
+           | |- context[@subevent _ ?F ?prf _ (|?e)%sum] => replace (@subevent _ F prf _ (|e)%sum) with (@subevent _ F _ _ e) by refl
+           end.
+        rewrite <- bind_trigger. resub. steps.
+        destruct s; ss.
+        {
+          destruct st_src0 as [rst_src0 pst_src0]; ss. destruct st_tgt0 as [rst_tgt0 pst_tgt0]; ss.
+          destruct p; ss.
+          - steps. instantiate (1:=100). gbase. eapply CIH0; ss; et.
+          - steps. instantiate (1:=100). gbase. eapply CIH0; ss; et.
+        }
+        { dependent destruction e.
+          - steps. unshelve esplits; et. instantiate (1:=100). steps. gbase. eapply CIH0; ss; et.
+          - steps. unshelve esplits; et. instantiate (1:=100). steps. gbase. eapply CIH0; ss; et.
+          - steps. unshelve esplits; et. instantiate (1:=100). steps. gbase. eapply CIH0; ss; et.
+        }
+      }
+      dependent destruction h.
+      rewrite <- bind_trigger. resub.
+      Opaque fun_to_src fun_to_mid.
+
+      destruct st_src0 as [rst_src0 pst_src0]; ss. destruct st_tgt0 as [rst_tgt0 pst_tgt0]; ss.
+      ired_both.
+      destruct tbr.
+      + (*** PURE CALL ***)
+        mred.
+        seal_left.
+        Ltac step := (mred; try _step; des_ifs_safe).
+        step; try by eapply OrdArith.lt_from_nat.
+        step; try by eapply OrdArith.lt_from_nat.
+        unseal_left.
+        step; try by eapply OrdArith.lt_from_nat.
+        instantiate (1:=(120 + formula (ord_pure x) + 100)%ord).
+        seal_left.
+
+        steps.
+        destruct rst_tgt0 as [mrs_tgt0 [|frs_tgt_hd frs_tgt_tl]]; ss.
+        { unseal_left. steps. }
+        steps.
+        unfold unwrapU. des_ifs; cycle 1.
+        { admit "unwrapN!!!!!!!!!!!!!!!!!!!!!!!!!!". }
+        steps.
+        unseal_left.
+        unfold ms_mid, mds_mid, SMod.to_mid in Heq. rewrite SMod.transl_fnsems in Heq.
+        unfold SMod.load_fnsems in Heq. apply find_some in Heq. des; ss. des_sumbool; subst.
+        rewrite in_flat_map in Heq. des; ss. rewrite in_flat_map in Heq0. des; ss. des_ifs. ss; des; ss; clarify.
+        rename Heq0 into INF. rename Heq into IN.
+        rename x1 into md0. fold sk in INF. fold sk in INF.
+        mred.
+        guclo ordC_spec. econs.
+        { instantiate (1:=(120 + (10 + C.myF x + 10))%ord).
+          rewrite <- ! OrdArith.add_assoc. eapply add_le_le; try refl. eapply OrdArith.le_from_nat; ss. lia. }
+        rename x into o1.
+        rewrite <- bind_bind.
+        rewrite <- bind_bind.
+        guclo bindC_spec. econs.
+        * (* guclo ordC_spec. econs. *)
+          (* { eapply OrdArith.add_base_r. } *)
+          (* gbase. eapply CIH; et. *)
+          gbase. hexploit CIH; et.
+          { instantiate (1:=(mrs_tgt0, ε :: frs_tgt_hd :: frs_tgt_tl, pst_tgt0)). instantiate (1:= (rst_src0, pst_tgt0)). ss. }
+          intro T. instantiate (2:=(ord_pure o1)) in T. ss.
+          mred.
+          (*** applying reduction in "T" begin ***)
+          (*** TODO: make prw "in" tactic ***)
+          revert T. pose (fun (x: Prop) (y: Prop) => (x -> y)) as myf.
+          match goal with | |- ?a -> ?b => replace (a -> b) with (myf a b) by refl end.
+          try Red.prw ltac:(IRed._red_gen) 2 2 0.
+          subst myf; cbn. intro T.
+          (*** applying reduction in "T" end ***)
+          eapply T.
+        * ii. des_ifs. destruct p, p0; ss. des; subst.
+          step; try by eapply OrdArith.lt_from_nat. steps.
+          destruct r1; ss.
+          des_ifs.
+          { unfold triggerNB. steps; try by eapply OrdArith.lt_from_nat. (*** TODO: fix tactic, don't unfold triggerNB ***) }
+          repeat (step; try by eapply OrdArith.lt_from_nat).
+          guclo ordC_spec. econs.
+          { instantiate (1:=100%ord). eapply OrdArith.le_from_nat; ss. lia. }
+          gbase. eapply CIH0. ss.
+      + (*** IMPURE CALL ***)
+        mred.
+        destruct rst_src0 as [mrs_src0 [|frs_src_hd frs_src_tl]]; ss.
+        { admit "SOMEHOW". }
+        mred. steps. instantiate (2:=(100 + (100 + 10) + 42)%ord). instantiate (1:=0%ord).
+        guclo ordC_spec. econs. { rewrite OrdArith.add_O_r. refl. }
+        destruct rst_tgt0 as [mrs_tgt0 [|frs_tgt_hd frs_tgt_tl]]; ss.
+        { steps. }
+        steps. unfold unwrapU at 2. des_ifs; cycle 1.
+        { admit "unwrapN!!!!!!!!!!!!!!!!!!". }
+        steps.
+        unfold unwrapU. des_ifs; cycle 1.
+        { steps. }
+        steps.
+
+        unfold ms_mid, mds_mid, SMod.to_mid in Heq. rewrite SMod.transl_fnsems in Heq.
+        unfold SMod.load_fnsems in Heq. apply find_some in Heq. des; ss. des_sumbool; subst.
+        rewrite in_flat_map in Heq. des; ss. rewrite in_flat_map in Heq1. des; ss. des_ifs. ss; des; ss; clarify.
+        rename Heq1 into INF. rename Heq into IN.
+        rename x0 into md0. fold sk in INF. fold sk in INF.
+
+        unfold ms_src, mds_src, SMod.to_src in Heq0. rewrite SMod.transl_fnsems in Heq0.
+        unfold SMod.load_fnsems in Heq0. apply find_some in Heq0. des; ss. des_sumbool; subst.
+        rewrite in_flat_map in Heq0. des; ss. rewrite in_flat_map in Heq1. des; ss. des_ifs. ss; des; ss; clarify.
+        rename Heq1 into INF0. rename Heq0 into IN0.
+        rename x0 into md1. fold sk in INF0. fold sk in INF0.
+
+        assert(md0 = md1); subst.
+        { admit "ez - uniqueness". }
+
+        assert(f = f0); subst.
+        { admit "ez - uniqueness". }
+
+        guclo ordC_spec. econs.
+        { eapply OrdArith.add_base_l. }
+        guclo bindC_spec.
+        econs.
+        * hexploit CIH; et; cycle 1.
+          { intro T. gbase. instantiate (3:=ord_top) in T. ss. eapply T. }
+          { ss. }
+        * ii; ss. des_ifs. steps. destruct p, p0; ss. des; subst.
+          steps. destruct r1; ss. des_ifs.
+          { unfold triggerNB. (step; try by eapply OrdArith.lt_from_nat). (*** TODO: fix tactic ***) }
+          destruct r0; ss. des_ifs. { admit "somehow". } steps.
+          instantiate (1:=100).
+          gbase. eapply CIH0 ;ss.
+  Unshelve.
+    all: try (by econs; et).
+    all: try (by exact Ord.O).
+    all: ss.
+  Unshelve.
+    all: try (by exact unit).
+  Qed.
+
+  Theorem adequacy_type_m2s: Beh.of_program (ModL.compile (Mod.add_list mds_mid)) <1=
+                             Beh.of_program (ModL.compile (Mod.add_list mds_src)).
+  Proof.
+    eapply adequacy_global.
+    exists (100)%ord. ss.
+    ginit.
+    { eapply cpn5_wcompat; eauto with paco. }
+    unfold ModSemL.initial_itr. Local Opaque ModSemL.prog. ss.
+    unfold ITree.map.
+    unfold assume.
+    steps.
+    instantiate (1:=(10 + (100 + 10) + 42)%ord).
+    esplits; et. { admit "ez - wf". } steps.
+    Local Transparent ModSemL.prog.
+    unfold ModSemL.prog at 4.
+    unfold ModSemL.prog at 2.
+    Local Opaque ModSemL.prog.
+    ss. steps.
+    (* Opaque ModSemL.initial_r_state. *)
+    (* Opaque ModSemL.initial_p_state. *)
+    fold ms_src. fold ms_mid.
+    set (rs_src0 := initial_r_state ms_src) in *.
+    set (rs_tgt0 := initial_r_state ms_mid) in *.
+    assert(exists mrs_src0 hd_src tl_src, rs_src0 = (mrs_src0, hd_src :: tl_src)).
+    { esplits. refl. }
+    assert(exists mrs_tgt0 hd_tgt tl_tgt, rs_tgt0 = (mrs_tgt0, hd_tgt :: tl_tgt)).
+    { esplits. refl. }
+    des. clearbody rs_src0 rs_tgt0. subst.
+    unfold unwrapU at 1. des_ifs; cycle 1.
+    { steps. }
+    unfold unwrapU. des_ifs; cycle 1.
+    { admit "unwrapN!!!!!!!!!!". }
+
+
+    unfold ms_mid, mds_mid, SMod.to_mid in Heq0. rewrite SMod.transl_fnsems in Heq0.
+    unfold SMod.load_fnsems in Heq0. apply find_some in Heq0. des; ss. des_sumbool; subst.
+    rewrite in_flat_map in Heq0. des; ss. rewrite in_flat_map in Heq2. des; ss. des_ifs. ss; des; ss; clarify. ss. subst.
+    rename Heq2 into INF. rename Heq0 into IN.
+    rename x into md0. fold sk in INF. fold sk in INF.
+
+    unfold ms_src, mds_src, SMod.to_src in Heq. rewrite SMod.transl_fnsems in Heq.
+    unfold SMod.load_fnsems in Heq. apply find_some in Heq. des; ss. destruct p; ss. des_sumbool; subst.
+    rewrite in_flat_map in Heq. des; ss. rewrite in_flat_map in Heq0. des; ss. des_ifs. ss; des; ss; clarify.
+    rename Heq0 into INF0. rename Heq into IN0.
+    rename x into md1. fold sk in INF0. fold sk in INF0.
+
+    assert(md0 = md1); subst.
+    { admit "ez - uniqueness". }
+    assert(f = f0).
+    { admit "ez - uniqueness". }
+    subst.
+    fold ms_src. fold ms_mid. fold p_src. fold p_mid.
+
+    steps.
+
+    match goal with
+    | [ |- gpaco6 _ _ _ _ _ _ _ _ ?i_src _ ] => remember i_src as tmp
+    end.
+    replace (([]: list val)↑) with (Any.pair ord_top↑ ([]: list val)↑) by admit "TODO".
+    subst tmp.
+
+    guclo ordC_spec. econs.
+    { eapply OrdArith.add_base_l. }
+    guclo bindC_spec.
+    econs.
+    - hexploit adequacy_type_aux; cycle 1.
+      { intro T. gfinal. right. instantiate (3:=ord_top) in T. ss. eapply T. }
+      ss. unfold ms_src, ms_mid. unfold initial_p_state.
+      apply func_ext. intro mn. unfold mds_src, mds_mid, SMod.to_src, SMod.to_mid.
+      rewrite ! SMod.transl_initial_mrs. ss.
+    - ii. rr in SIM. des_ifs. des; ss. subst. r in SIM. des_ifs. steps.
+  Unshelve.
+    all: ss.
+    all: try (by exact Ord.O).
+    all: try (by econs; et).
+  Qed.
+
+End CANCEL.
+
+Require Import Coqlib.
+Require Import Universe.
+Require Import STS.
+Require Import Behavior.
+Require Import ModSem.
+Import ModSemL.
+Require Import Skeleton.
+Require Import PCM.
+Require Import Any.
+Require Import HoareDef.
+Require Import SimSTS.
+Require Import SimGlobal.
+Require Import HoareDef.
+From Ordinal Require Import Ordinal Arithmetic.
+
+Set Implicit Arguments.
+
+
+
+
+
+
+
+
+
+
+
+
+
+
+
+
+
+
+
+
+
+
+
+
+
+
+
+
+
+
+
+
+
+Lemma add_le_lt: forall x0 x1 y0 y1, (x0 <= x1)%ord -> (y0 < y1)%ord -> (x0 + y0 < x1 + y1)%ord.
+Proof.
+  i.
+  eapply Ord.le_lt_lt.
+  - eapply OrdArith.le_add_l; et.
+  - eapply OrdArith.lt_add_r; et.
+Qed.
+
+Lemma add_le_le: forall x0 x1 y0 y1, (x0 <= x1)%ord -> (y0 <= y1)%ord -> (x0 + y0 <= x1 + y1)%ord.
+Proof.
+  i.
+  etrans.
+  - eapply OrdArith.le_add_r; et.
+  - eapply OrdArith.le_add_l; et.
+Qed.
+
+Lemma mul_le_lt: forall x0 x1 y0 y1, (0 < x1)%ord -> (x0 <= x1)%ord -> (y0 < y1)%ord -> (x0 * y0 < x1 * y1)%ord.
+Proof.
+  i.
+  eapply Ord.le_lt_lt.
+  - eapply OrdArith.le_mult_l; et.
+  - eapply OrdArith.lt_mult_r; et.
+Qed.
+
+Lemma mult_le_le: forall x0 x1 y0 y1, (x0 <= x1)%ord -> (y0 <= y1)%ord -> (x0 * y0 <= x1 * y1)%ord.
+Proof.
+  i.
+  etrans.
+  - eapply OrdArith.le_mult_l; et.
+  - eapply OrdArith.le_mult_r; et.
+Qed.
+
+Lemma expn_pos: forall base o, (1 <= base ^ o)%ord.
+Proof. i. rewrite Ord.from_nat_S. eapply Ord.S_supremum. eapply OrdArith.expn_pos. Qed.
+
+Lemma add_one_lt: forall o0 o1, (o0 < o1)%ord -> (o0 + 1 <= o1)%ord.
+Proof.
+  i.
+  rewrite Ord.from_nat_S.
+  rewrite OrdArith.add_S.
+  rewrite OrdArith.add_O_r.
+  eapply Ord.S_supremum; et.
+Qed.
+
+
+
+
+
+
+Module Type PARAM.
+  Parameter c: Ord.t.
+  Parameter d: Ord.t.
+  Parameter e: Ord.t.
+  Parameter f: Ord.t.
+End PARAM.
+
+Module Construction (P: PARAM).
+  Include P.
+
+  Section CONSTRUCTION.
+
+  Let alpha := (f + 3 + d + e)%ord.
+  (* Let alpha_d: ((1 + d) <= alpha)%ord. *)
+  (* Proof. unfold alpha. rewrite <- OrdArith.add_O_r at 1. eapply add_le_le; try refl. eapply Ord.O_is_O. Qed. *)
+  Let alpha_e: (e <= alpha)%ord.
+  Proof.
+    unfold alpha.
+    eapply OrdArith.add_base_r.
+    (* etrans; [eapply OrdArith.add_base_l|]. *)
+    (* etrans; [eapply OrdArith.add_base_r|]. *)
+    (* rewrite <- OrdArith.add_assoc. rewrite OrdArith.add_assoc. refl. *)
+  Qed.
+
+  Let alpha_d: (f + 3 + d <= alpha)%ord.
+  Proof.
+    unfold alpha.
+    eapply OrdArith.add_base_l.
+    (* etrans; [eapply OrdArith.add_base_l|]. *)
+    (* etrans; [eapply OrdArith.add_base_r|]. *)
+    (* rewrite <- OrdArith.add_assoc. *)
+    (* eapply add_le_le; try refl. *)
+    (* rewrite <- OrdArith.add_assoc. *)
+    (* refl. *)
+  Qed.
+
+  Definition myF (o0: Ord.t): Ord.t := ((alpha * kappa + c) ^ (o0 + 1))%ord.
+  Definition myG (o0 m0: Ord.t): Ord.t := ((alpha * kappa + c) ^ (o0) * alpha * m0)%ord.
+  Definition myH (o0: Ord.t): Ord.t := ((alpha * kappa + c) ^ (o0) * 3)%ord.
+
+  (***
+                         (myG o0 kappa + d <= myF o0)
+  (AM: (m1 < m0)%ord) -> (myG o0 m1 + myH o0 + c <= myG o0 m0)%ord
+  (O: (o1 < o0)%ord)  -> (myF o1 + e <= myH o0)%ord
+   ***)
+
+  Let NZERO: (Ord.O < alpha * kappa + c)%ord.
+  Proof.
+    unfold alpha.
+
+    assert(T: (1 < f + 3 + d + e)%ord).
+    { assert(U: (1 + 1 <= (Ord.from_nat 3))%ord).
+      { rewrite <- OrdArith.add_from_nat. ss. eapply OrdArith.le_from_nat; et. }
+      eapply Ord.lt_le_lt; cycle 1.
+      { rewrite <- U. refl. }
+      rewrite ! OrdArith.add_assoc.
+      eapply Ord.lt_le_lt; cycle 1.
+      { eapply OrdArith.add_base_r. }
+      eapply OrdArith.add_lt_l.
+      rewrite Ord.from_nat_S at 1.
+      eapply Ord.lt_le_lt.
+      { instantiate (1:=1%ord). rewrite Ord.from_nat_S. eapply Ord.S_pos. }
+      { rewrite Ord.from_nat_S. eapply OrdArith.add_base_l. }
+    }
+
+    eapply Ord.lt_le_lt; cycle 1.
+    { eapply OrdArith.add_base_l. }
+    rewrite <- OrdArith.mult_1_r.
+    eapply Ord.le_lt_lt; cycle 1.
+    { instantiate (1:=((f + 3 + d + e) * 1)%ord).
+      eapply OrdArith.lt_mult_r.
+      - eauto with ord_kappa.
+      - rewrite <- T. replace (Ord.from_nat 1) with (Ord.S Ord.O) by ss. eapply Ord.S_pos. }
+    eapply mult_le_le.
+    - eapply Ord.O_is_O.
+    - refl.
+  Qed.
+
+  Global Program Instance myG_proper: Proper (Ord.le ==> Ord.le ==> Ord.le) (myG).
+  Next Obligation.
+    ii. unfold myG.
+    rewrite <- H0.
+    eapply mult_le_le; et; try refl.
+    eapply mult_le_le; et; try refl.
+    rewrite <- H. refl.
+  Qed.
+
+  Theorem my_thm1: forall o0, (myG o0 kappa + c <= myF o0)%ord.
+  Proof.
+    i. unfold myF, myG, myH.
+    rewrite OrdArith.expn_add; et.
+    rewrite OrdArith.expn_1_r; et.
+    rewrite OrdArith.mult_dist.
+    eapply add_le_le.
+    - rewrite <- OrdArith.mult_assoc. refl.
+    - rewrite <- (OrdArith.mult_1_l) at 1. eapply mult_le_le; try refl. eapply expn_pos.
+    (* OrdArith.add *)
+    (* OrdArith.mult *)
+    (* OrdArith.expn *)
+  Qed.
+
+  Theorem my_thm3
+          o0 o1
+          (O: (o1 < o0)%ord)
+    :
+      (myF o1 + e <= myH o0)%ord
+  .
+  Proof.
+    unfold myF, myG, myH.
+    eapply add_one_lt in O.
+    rewrite <- O.
+    rewrite OrdArith.expn_add; et.
+    rewrite OrdArith.expn_1_r; et.
+    assert(T: (1 + 1 <= 3)%ord).
+    { rewrite <- OrdArith.add_from_nat. ss. eapply OrdArith.le_from_nat; et. }
+    rewrite <- T.
+    rewrite OrdArith.mult_dist with (o2:=1).
+    rewrite OrdArith.mult_1_r.
+    eapply add_le_le; try refl.
+    rewrite <- (OrdArith.mult_1_l) at 1.
+    eapply mult_le_le.
+    { eapply expn_pos. }
+    rewrite <- alpha_e.
+    etrans; [|eapply OrdArith.add_base_l].
+    rewrite <- (OrdArith.mult_1_r) at 1.
+    eapply mult_le_le; try refl.
+    eapply Ord.lt_le.
+    eauto with ord_kappa.
+  Qed.
+
+  Theorem my_thm2
+          o0 m0 m1
+          (AM: (m1 < m0)%ord)
+    :
+      (myG o0 m1 + f + myH o0 + d <= myG o0 m0)%ord
+  .
+  Proof.
+    unfold myF, myG, myH.
+    eapply add_one_lt in AM.
+    rewrite <- AM.
+    rewrite OrdArith.mult_dist.
+    rewrite OrdArith.mult_1_r.
+    rewrite OrdArith.add_assoc.
+    rewrite OrdArith.add_assoc.
+    eapply add_le_le; try refl.
+    rewrite <- alpha_d at 3.
+    rewrite OrdArith.mult_dist.
+    rewrite OrdArith.mult_dist.
+    rewrite <- OrdArith.add_assoc.
+    eapply add_le_le; try refl; cycle 1.
+    { rewrite <- (OrdArith.mult_1_l) at 1. eapply mult_le_le; try refl. eapply expn_pos. }
+    eapply add_le_le; try refl; cycle 1.
+    { rewrite <- (OrdArith.mult_1_l) at 1. eapply mult_le_le; try refl. eapply expn_pos. }
+  Qed.
+
+  End CONSTRUCTION.
+
+End Construction.
+
+
+Module MyParam <: PARAM.
+  Definition d: Ord.t := 50%ord.
+  Definition c: Ord.t := (d + 30)%ord.
+  Definition e: Ord.t := 50%ord.
+  Definition f: Ord.t := (d + 10)%ord.
+End MyParam.
+
+Module C := (Construction MyParam).
+
+
+
+
+
+
+
+
+
+
+
+
+(* Lemma upcast_ty: forall T (v: T), Any.ty v↑ = T. admit "ez". Qed. *)
+(* Lemma upcast_val: forall T (v: T), Any.val v↑ ~= v. admit "ez". Qed. *)
+
+
+
+
+
+
+Inductive opair: Type := mk_opair { ofst: Ord.t; osnd: Ord.t }.
+(* Definition opair_lt: opair -> opair -> Prop := fun '(mk_opair x0 x1) '(mk_opair y0 y1) => (x0 < y0)%ord \/ (x0 == y0 /\ x1 < y1)%ord. *)
+Inductive opair_lt: opair -> opair -> Prop :=
+| intro_opair_lt
+    x0 x1 y0 y1
+    (LT: (x0 < y0)%ord \/ (x0 == y0 /\ x1 < y1)%ord)
+  :
+    opair_lt (mk_opair x0 x1) (mk_opair y0 y1)
+.
+Theorem wf_opair_lt: well_founded opair_lt.
+Proof.
+  ii. destruct a.
+  revert osnd0. pattern ofst0. eapply well_founded_ind. { eapply Ord.lt_well_founded. } clear ofst0. intros ? IH0.
+  intro. generalize dependent x. pattern osnd0. eapply well_founded_ind. { eapply Ord.lt_well_founded. } clear osnd0. intros ? IH1.
+  econs. i. inv H. des.
+  { eapply IH0; et. }
+  { eapply IH1; et. i. eapply IH0; et. rewrite <- LT. ss. }
+Qed.
+
+
+
+
+
+
+
+
+
+
+
+Section CANCEL.
+
+  (*** execute following commands in emacs (by C-x C-e)
+     (progn (highlight-phrase "Any" 'hi-red-b) (highlight-phrase "Any_src" 'hi-green-b) (highlight-phrase "Any_tgt" 'hi-blue-b)
+            (highlight-phrase "Any_mid" 'hi-light-green-b)
+            (highlight-phrase "Y" 'hi-green-b) (highlight-phrase "Z" 'hi-green-b)) ***)
+  Let Any_src := Any.t. (*** src argument (e.g., List nat) ***)
+  Let Any_mid := Any.t. (*** src argument (e.g., List nat) ***)
+  Let Any_tgt := Any.t. (*** tgt argument (i.e., list val) ***)
+
+
+
+  Context `{Σ: GRA.t}.
+
+  Variable mds: list SMod.t.
+
+  Let sk: Sk.t := fold_right Sk.add Sk.unit (List.map SMod.sk mds).
+  (* Let skenv: SkEnv.t := Sk.load_skenv sk. *)
+  Let mss: list SModSem.t := (List.map ((flip SMod.get_modsem) sk) mds).
+  Let sbtb: list (gname * fspecbody) := (List.flat_map (SModSem.fnsems) mss).
+  Let stb: list (gname * fspec) := List.map (fun '(fn, fs) => (fn, fs.(fsb_fspec))) sbtb.
+
+  Let mds_src: list Mod.t := List.map (SMod.to_src) mds.
+  Let mds_mid: list Mod.t := List.map (SMod.to_mid stb) mds.
+
+
+
+  Let W: Type := (r_state * p_state).
+  (* Let wf: Ord.t -> W -> W -> Prop := top3. *)
+
+  Opaque EventsL.interp_Es.
+
+  Let ms_src: ModSemL.t := ModL.enclose (Mod.add_list mds_src).
+  Let ms_mid: ModSemL.t := ModL.enclose (Mod.add_list mds_mid).
+
+  Let p_src := ModSemL.prog ms_src.
+  Let p_mid := ModSemL.prog ms_mid.
+
+  Ltac _step :=
+    match goal with
+    (*** terminal cases ***)
+    | [ |- gpaco5 _ _ _ _ _ _ _ (triggerUB >>= _) _ ] =>
+      unfold triggerUB; mred; _step; ss; fail
+    | [ |- gpaco5 _ _ _ _ _ _ _ (triggerNB >>= _) _ ] =>
+      exfalso
+    | [ |- gpaco5 _ _ _ _ _ _ _ _ (triggerUB >>= _) ] =>
+      exfalso
+    | [ |- gpaco5 _ _ _ _ _ _ _ _ (triggerNB >>= _) ] =>
+      unfold triggerNB; mred; _step; ss; fail
+
+    (*** assume/guarantee ***)
+    | [ |- gpaco5 _ _ _ _ _ _ _ (assume ?P ;;; _) _ ] =>
+      let tvar := fresh "tmp" in
+      let thyp := fresh "TMP" in
+      remember (assume P) as tvar eqn:thyp; unfold assume in thyp; subst tvar
+    | [ |- gpaco5 _ _ _ _ _ _ _ (guarantee ?P ;;; _) _ ] =>
+      let tvar := fresh "tmp" in
+      let thyp := fresh "TMP" in
+      remember (guarantee P) as tvar eqn:thyp; unfold guarantee in thyp; subst tvar
+    | [ |- gpaco5 _ _ _ _ _ _ _ _ (assume ?P ;;; _) ] =>
+      let tvar := fresh "tmp" in
+      let thyp := fresh "TMP" in
+      remember (assume P) as tvar eqn:thyp; unfold assume in thyp; subst tvar
+    | [ |- gpaco5 _ _ _ _ _ _ _ _ (guarantee ?P ;;; _) ] =>
+      let tvar := fresh "tmp" in
+      let thyp := fresh "TMP" in
+      remember (guarantee P) as tvar eqn:thyp; unfold guarantee in thyp; subst tvar
+
+    (*** default cases ***)
+    | _ =>
+      (gstep; econs; eauto; try (eapply add_le_lt; [refl|eapply OrdArith.lt_from_nat; ss]);
+       (*** some post-processing ***)
+       i;
+       try match goal with
+           | [ |- (eq ==> _)%signature _ _ ] =>
+             let v_src := fresh "v_src" in
+             let v_tgt := fresh "v_tgt" in
+             intros v_src v_tgt ?; subst v_tgt
+           end)
+    end
+  .
+
+  Ltac steps := repeat (mred; try _step; des_ifs_safe).
+
+Let adequacy_type_aux__APC:
+    forall at_most o0 mn
+           st_src0 st_tgt0
+    ,
+      simg (fun _ '(st_tgt1, _) => st_tgt1 = st_tgt0)
+           (C.myG o0 at_most + C.d)%ord (Ret (st_src0, tt))
+           (EventsL.interp_Es p_mid (transl_all mn (interp_hCallE_mid stb (ord_pure o0) (_APC at_most))) st_tgt0)
+  .
+  Proof.
+    ginit.
+    { i. eapply cpn5_wcompat; eauto with paco. }
+    (* induction *)
+    intros ? ?. remember (mk_opair o0 at_most) as fuel. move fuel at top. revert at_most o0 Heqfuel.
+    pattern fuel. eapply well_founded_induction. { eapply wf_opair_lt. } clear fuel.
+    intros fuel IH. i.
+
+    rewrite unfold_APC. destruct st_tgt0 as [rst_tgt0 pst_tgt0]. steps.
+    destruct x.
+    { steps. }
+    steps. destruct (alist_find s stb) eqn:EQ; ss.
+    2: { steps. }
+    destruct rst_tgt0 as [mrs_tgt0 [|frs_hd frs_tl]]; ss.
+    { steps. destruct (Any.downcast t0); steps. }
+    steps. destruct (Any.downcast t0); ss.
+    2:{ steps. }
+    steps. unfold unwrapU. des_ifs; cycle 1.
+    { exfalso. hexploit (stb_find_iff s). rewrite EQ. rewrite Heq. clear. intuition. }
+    unfold ms_mid, mds_mid, SMod.to_mid in Heq. rewrite SMod.transl_fnsems in Heq.
+    unfold SMod.load_fnsems in Heq. apply find_some in Heq. des; ss. des_sumbool; subst.
+    rewrite in_flat_map in Heq. des; ss. rewrite in_flat_map in Heq0. des; ss. des_ifs. ss; des; ss; clarify.
+    rename Heq0 into INF. rename Heq into IN.
+    rename x3 into md0. fold sk in INF. fold sk in INF.
+    unfold fun_to_mid.
+    steps. assert (f0.(fsb_fspec) = f).
+    { admit "fspec table". }
+    subst. rewrite Any.upcast_downcast. steps.
+    guclo ordC_spec. econs.
+    { eapply OrdArith.add_base_l. }
+    guclo ordC_spec. econs.
+    { eapply C.my_thm2; et. }
+    guclo ordC_spec. econs.
+    { rewrite OrdArith.add_assoc. refl. }
+    rewrite idK_spec at 1.
+    guclo bindC_spec. econs.
+    { unfold APC. gstep. mred. eapply simg_chooseR; et; [_ord_step|]. i. steps.
+      guclo ordC_spec. econs.
+      { instantiate (1:=(C.myG x1 x3 + C.d)%ord).
+        rewrite <- C.my_thm3; et.
+        rewrite <- C.my_thm1; et.
+        rewrite OrdArith.add_assoc.
+        rewrite OrdArith.add_assoc.
+        eapply add_le_le.
+        - eapply Ord.lt_le in x4. rewrite <- x4. refl.
+        - etrans; [|eapply OrdArith.add_base_l]. etrans; [|eapply OrdArith.add_base_l]. refl.
+      }
+      eapply IH; auto. econs. left. auto.
+    }
+
+    i. ss. destruct vret_tgt as [? []]. destruct vret_src as [? []]. ss. des; subst.
+    unfold idK. unfold C.f.
+    guclo ordC_spec. econs.
+    { rewrite <- OrdArith.add_assoc. refl. }
+    steps.
+    guclo ordC_spec. econs.
+    { eapply OrdArith.add_base_l. }
+    { eapply IH; et. econs; et. right; split; et. refl. }
+  Qed.
+
+
+  Let adequacy_type_aux__APC:
+    forall at_most o0 mn
+           st_src0 st_tgt0
+    ,
+      simg (fun _ '(st_tgt1, _) => st_tgt1 = st_tgt0)
+           (C.myG o0 at_most + C.d)%ord
+           (Ret (st_src0, tt))
+           (EventsL.interp_Es p_mid (transl_all mn (interp_hCallE_mid stb (ord_pure o0) (_APC at_most))) st_tgt0)
+  .
+  Proof.
+    ginit.
+    { i. eapply cpn5_wcompat; eauto with paco. }
+    intros ? ?. remember (mk_opair o0 at_most) as fuel. move fuel at top. revert at_most o0 Heqfuel.
+    pattern fuel. eapply well_founded_induction. { eapply wf_opair_lt. } clear fuel.
+    intros fuel IH.
+    i. rewrite unfold_APC.
+    destruct st_tgt0 as [rst_tgt0 pst_tgt0]. destruct rst_tgt0 as [mrs_tgt0 [|frs_hd frs_tl]]; ss.
+    { admit "-----------------------------------it should not happen...". }
+    unfold C.d.
+    steps.
+    destruct x.
+    { steps. }
+    steps.
+    (*************** TODO: define force_l/r *************)
+    unfold unwrapU. des_ifs; cycle 1.
+    { admit "-----------------------------------FINDF: make it to unwrapN". }
+    steps.
+    unfold ms_mid, mds_mid, SMod.to_mid in Heq. rewrite SMod.transl_fnsems in Heq.
+    unfold SMod.load_fnsems in Heq. apply find_some in Heq. des; ss. des_sumbool; subst.
+    rewrite in_flat_map in Heq. des; ss. rewrite in_flat_map in Heq0. des; ss. des_ifs. ss; des; ss; clarify.
+    rename Heq0 into INF. rename Heq into IN.
+    rename x3 into md0. fold sk in INF. fold sk in INF.
+    unfold fun_to_mid.
+    steps.
+    unfold unwrapN.
+    des_ifs; cycle 1.
+    { steps. }
+    steps.
+    des_ifs_safe.
+    eapply pair_downcast_lemma in Heq. des. subst.
+    des_ifs; ss.
+    steps.
+
+    guclo ordC_spec. econs.
+    { eapply OrdArith.add_base_l. }
+    guclo ordC_spec. econs.
+    { eapply C.my_thm2; et. }
+    guclo ordC_spec. econs.
+    { rewrite OrdArith.add_assoc. refl. }
+    rewrite idK_spec at 1.
+    guclo bindC_spec. econs.
+    {
+      Local Transparent APC.
+      unfold APC.
+      steps.
+      guclo ordC_spec. econs.
+      { instantiate (1:=(C.myG x1 x3 + C.d)%ord).
+        rewrite <- C.my_thm3; et.
+        rewrite <- C.my_thm1; et.
+        rewrite OrdArith.add_assoc.
+        rewrite OrdArith.add_assoc.
+        eapply add_le_le.
+        - eapply Ord.lt_le in x4. rewrite <- x4. refl.
+        - etrans; [|eapply OrdArith.add_base_l]. etrans; [|eapply OrdArith.add_base_l]. refl.
+      }
+      eapply IH; et. econs; et.
+    }
+    i. ss. des_ifs. destruct vret_src; ss. repeat des_u. unfold idK.
+    unfold C.f.
+    guclo ordC_spec. econs.
+    { rewrite <- OrdArith.add_assoc. refl. }
+    steps.
+    guclo ordC_spec. econs; cycle 1.
+    { eapply IH; et. econs; et. right; split; et. refl. }
+    { eapply OrdArith.add_base_l. }
+  Qed.
+
+  Let adequacy_type_aux_APC:
+    forall o0 st_src0 st_tgt0 mn
+    ,
+      simg (fun _ '(st_tgt1, _) => st_tgt1 = st_tgt0)
+           (C.myF o0)%ord (Ret (st_src0, tt))
+           (EventsL.interp_Es p_mid (transl_all mn (interp_hCallE_mid (ord_pure o0) APC)) st_tgt0)
+  .
+  Proof.
+    ginit.
+    { i. eapply cpn5_wcompat; eauto with paco. }
+    i. unfold APC.
+    guclo ordC_spec. econs.
+    { rewrite <- C.my_thm1. refl. }
+    unfold C.c.
+    guclo ordC_spec. econs.
+    { rewrite <- OrdArith.add_assoc. refl. }
+    steps.
+    guclo ordC_spec. econs.
+    { etrans; [|eapply OrdArith.add_base_l]. eapply add_le_le; [|refl].
+      instantiate (1:=C.myG o0 x).
+      eapply Ord.lt_le in x0. rewrite <- x0. refl. }
+    gfinal. right.
+    eapply adequacy_type_aux__APC.
+  Qed.
+
+  Lemma idK_spec2: forall E A B (a: A) (itr: itree E B), itr = Ret a >>= fun _ => itr. Proof. { i. ired. ss. } Qed.
+
+  Definition formula (o0: ord): Ord.t :=
+    match o0 with
+    | ord_pure o0 => (10 + C.myF o0)%ord
+    | ord_top => 100%ord
+    end
+  .
+
+  Let wf: W -> W -> Prop := fun '(_, pst_src0) '(_, pst_tgt0) => pst_src0 = pst_tgt0.
+  Let wf': forall {X}, (W * X)%type -> (W * X)%type -> Prop := (fun _ '(st_src0, rv_src) '(st_tgt0, rv_tgt) => wf st_src0 st_tgt0 /\ rv_src = rv_tgt).
+
+  Let adequacy_type_aux:
+    forall
+      AA AR
+      args
+      o0
+      body st_src0 st_tgt0 mn
+      (SIM: wf st_src0 st_tgt0)
+    ,
+      simg wf'
+           (formula o0 + 10)%ord
+           (* (if is_pure o0 then trigger (Choose _) else (interp_Es p_src ((fun_to_src (AA:=AA) (AR:=AR) body) args↑) st0)) *)
+           (EventsL.interp_Es p_src (transl_all mn (if is_pure o0 then trigger (Choose _) else ((fun_to_src (AA:=AA) (AR:=AR) body) args))) st_src0)
+           (EventsL.interp_Es p_mid (transl_all mn ((fun_to_mid body) (Any.pair o0↑ args))) st_tgt0)
+  .
+  Proof.
+    ginit.
+    { i. eapply cpn5_wcompat; eauto with paco. }
+    gcofix CIH. i.
+    unfold fun_to_src, fun_to_mid. steps. unfold unwrapN.
+    destruct (Any.downcast (Any.pair (Any.upcast o0) args)) eqn:T; cycle 1.
+    { steps. }
+    destruct p.
+    eapply pair_downcast_lemma in T. des; subst; ss. eapply Any.downcast_upcast in T0. des; subst.
+    unfold body_to_src, cfun. steps. rewrite Any.upcast_downcast. ss. steps.
+    destruct o; ss.
+    - (*** PURE ***)
+      seal_left.
+      steps.
+      unseal_left.
+      erewrite idK_spec2 at 1.
+      guclo ordC_spec. econs.
+      { eapply OrdArith.add_base_l. }
+      guclo bindC_spec.
+      econs.
+      { gfinal. right. eapply paco5_mon. { eapply adequacy_type_aux_APC. } ii; ss. }
+      ii; ss. des_ifs. des_u.
+      steps. esplits; eauto. steps.
+    - (*** IMPURE ***)
+      steps. unfold body_to_mid.
+      abstr (body a) itr. clear body a AA.
+
+      guclo ordC_spec. econs.
+      { instantiate (1:=(10 + 100)%ord). rewrite <- ! OrdArith.add_from_nat. ss. refl. }
+      (* { instantiate (1:=(1 + 99)%ord). rewrite <- OrdArith.add_from_nat. ss. refl. } *)
+      guclo bindC_spec. eapply bindR_intro with (RR:=wf'); cycle 1.
+      { ii. subst. des_ifs. steps. r in SIM0. des; subst; ss. }
+
+      revert_until CIH. gcofix CIH0. i.
+
+      ides itr.
+      { steps. }
+      { steps. gbase. eapply CIH0; ss. }
+      destruct e; cycle 1.
+      {
+
+        (*** TODO: remove redundancy with Hoareproof0 ***)
+  Ltac resub :=
+    repeat multimatch goal with
+           | |- context[ITree.trigger ?e] =>
+             match e with
+             | subevent _ _ => idtac
+             | _ => replace (ITree.trigger e) with (trigger e) by refl
+             end
+           | |- context[@subevent _ ?F ?prf _ (?e|)%sum] => replace (@subevent _ F prf _ (e|)%sum) with (@subevent _ F _ _ e) by refl
+           | |- context[@subevent _ ?F ?prf _ (|?e)%sum] => replace (@subevent _ F prf _ (|e)%sum) with (@subevent _ F _ _ e) by refl
+           end.
+        rewrite <- bind_trigger. resub. steps.
+        destruct s; ss.
+        {
+          destruct st_src0 as [rst_src0 pst_src0]; ss. destruct st_tgt0 as [rst_tgt0 pst_tgt0]; ss.
+          destruct p; ss.
+          - steps. instantiate (1:=100). gbase. eapply CIH0; ss; et.
+          - steps. instantiate (1:=100). gbase. eapply CIH0; ss; et.
+        }
+        { dependent destruction e.
+          - steps. unshelve esplits; et. instantiate (1:=100). steps. gbase. eapply CIH0; ss; et.
+          - steps. unshelve esplits; et. instantiate (1:=100). steps. gbase. eapply CIH0; ss; et.
+          - steps. unshelve esplits; et. instantiate (1:=100). steps. gbase. eapply CIH0; ss; et.
+        }
+      }
+      dependent destruction h.
+      rewrite <- bind_trigger. resub.
+      Opaque fun_to_src fun_to_mid.
+
+      destruct st_src0 as [rst_src0 pst_src0]; ss. destruct st_tgt0 as [rst_tgt0 pst_tgt0]; ss.
+      ired_both.
+      destruct tbr.
+      + (*** PURE CALL ***)
+        mred.
+        seal_left.
+        Ltac step := (mred; try _step; des_ifs_safe).
+        step; try by eapply OrdArith.lt_from_nat.
+        step; try by eapply OrdArith.lt_from_nat.
+        unseal_left.
+        step; try by eapply OrdArith.lt_from_nat.
+        instantiate (1:=(120 + formula (ord_pure x) + 100)%ord).
+        seal_left.
+
+        steps.
+        destruct rst_tgt0 as [mrs_tgt0 [|frs_tgt_hd frs_tgt_tl]]; ss.
+        { unseal_left. steps. }
+        steps.
+        unfold unwrapU. des_ifs; cycle 1.
+        { admit "unwrapN!!!!!!!!!!!!!!!!!!!!!!!!!!". }
+        steps.
+        unseal_left.
+        unfold ms_mid, mds_mid, SMod.to_mid in Heq. rewrite SMod.transl_fnsems in Heq.
+        unfold SMod.load_fnsems in Heq. apply find_some in Heq. des; ss. des_sumbool; subst.
+        rewrite in_flat_map in Heq. des; ss. rewrite in_flat_map in Heq0. des; ss. des_ifs. ss; des; ss; clarify.
+        rename Heq0 into INF. rename Heq into IN.
+        rename x1 into md0. fold sk in INF. fold sk in INF.
+        mred.
+        guclo ordC_spec. econs.
+        { instantiate (1:=(120 + (10 + C.myF x + 10))%ord).
+          rewrite <- ! OrdArith.add_assoc. eapply add_le_le; try refl. eapply OrdArith.le_from_nat; ss. lia. }
+        rename x into o1.
+        rewrite <- bind_bind.
+        rewrite <- bind_bind.
+        guclo bindC_spec. econs.
+        * (* guclo ordC_spec. econs. *)
+          (* { eapply OrdArith.add_base_r. } *)
+          (* gbase. eapply CIH; et. *)
+          gbase. hexploit CIH; et.
+          { instantiate (1:=(mrs_tgt0, ε :: frs_tgt_hd :: frs_tgt_tl, pst_tgt0)). instantiate (1:= (rst_src0, pst_tgt0)). ss. }
+          intro T. instantiate (2:=(ord_pure o1)) in T. ss.
+          mred.
+          (*** applying reduction in "T" begin ***)
+          (*** TODO: make prw "in" tactic ***)
+          revert T. pose (fun (x: Prop) (y: Prop) => (x -> y)) as myf.
+          match goal with | |- ?a -> ?b => replace (a -> b) with (myf a b) by refl end.
+          try Red.prw ltac:(IRed._red_gen) 2 2 0.
+          subst myf; cbn. intro T.
+          (*** applying reduction in "T" end ***)
+          eapply T.
+        * ii. des_ifs. destruct p, p0; ss. des; subst.
+          step; try by eapply OrdArith.lt_from_nat. steps.
+          destruct r1; ss.
+          des_ifs.
+          { unfold triggerNB. steps; try by eapply OrdArith.lt_from_nat. (*** TODO: fix tactic, don't unfold triggerNB ***) }
+          repeat (step; try by eapply OrdArith.lt_from_nat).
+          guclo ordC_spec. econs.
+          { instantiate (1:=100%ord). eapply OrdArith.le_from_nat; ss. lia. }
+          gbase. eapply CIH0. ss.
+      + (*** IMPURE CALL ***)
+        mred.
+        destruct rst_src0 as [mrs_src0 [|frs_src_hd frs_src_tl]]; ss.
+        { admit "SOMEHOW". }
+        mred. steps. instantiate (2:=(100 + (100 + 10) + 42)%ord). instantiate (1:=0%ord).
+        guclo ordC_spec. econs. { rewrite OrdArith.add_O_r. refl. }
+        destruct rst_tgt0 as [mrs_tgt0 [|frs_tgt_hd frs_tgt_tl]]; ss.
+        { steps. }
+        steps. unfold unwrapU at 2. des_ifs; cycle 1.
+        { admit "unwrapN!!!!!!!!!!!!!!!!!!". }
+        steps.
+        unfold unwrapU. des_ifs; cycle 1.
+        { steps. }
+        steps.
+
+        unfold ms_mid, mds_mid, SMod.to_mid in Heq. rewrite SMod.transl_fnsems in Heq.
+        unfold SMod.load_fnsems in Heq. apply find_some in Heq. des; ss. des_sumbool; subst.
+        rewrite in_flat_map in Heq. des; ss. rewrite in_flat_map in Heq1. des; ss. des_ifs. ss; des; ss; clarify.
+        rename Heq1 into INF. rename Heq into IN.
+        rename x0 into md0. fold sk in INF. fold sk in INF.
+
+        unfold ms_src, mds_src, SMod.to_src in Heq0. rewrite SMod.transl_fnsems in Heq0.
+        unfold SMod.load_fnsems in Heq0. apply find_some in Heq0. des; ss. des_sumbool; subst.
+        rewrite in_flat_map in Heq0. des; ss. rewrite in_flat_map in Heq1. des; ss. des_ifs. ss; des; ss; clarify.
+        rename Heq1 into INF0. rename Heq0 into IN0.
+        rename x0 into md1. fold sk in INF0. fold sk in INF0.
+
+        assert(md0 = md1); subst.
+        { admit "ez - uniqueness". }
+
+        assert(f = f0); subst.
+        { admit "ez - uniqueness". }
+
+        guclo ordC_spec. econs.
+        { eapply OrdArith.add_base_l. }
+        guclo bindC_spec.
+        econs.
+        * hexploit CIH; et; cycle 1.
+          { intro T. gbase. instantiate (3:=ord_top) in T. ss. eapply T. }
+          { ss. }
+        * ii; ss. des_ifs. steps. destruct p, p0; ss. des; subst.
+          steps. destruct r1; ss. des_ifs.
+          { unfold triggerNB. (step; try by eapply OrdArith.lt_from_nat). (*** TODO: fix tactic ***) }
+          destruct r0; ss. des_ifs. { admit "somehow". } steps.
+          instantiate (1:=100).
+          gbase. eapply CIH0 ;ss.
+  Unshelve.
+    all: try (by econs; et).
+    all: try (by exact Ord.O).
+    all: ss.
+  Unshelve.
+    all: try (by exact unit).
+  Qed.
+
+  Theorem adequacy_type_m2s: Beh.of_program (ModL.compile (Mod.add_list mds_mid)) <1=
+                             Beh.of_program (ModL.compile (Mod.add_list mds_src)).
+  Proof.
+    eapply adequacy_global.
+    exists (100)%ord. ss.
+    ginit.
+    { eapply cpn5_wcompat; eauto with paco. }
+    unfold ModSemL.initial_itr. Local Opaque ModSemL.prog. ss.
+    unfold ITree.map.
+    unfold assume.
+    steps.
+    instantiate (1:=(10 + (100 + 10) + 42)%ord).
+    esplits; et. { admit "ez - wf". } steps.
+    Local Transparent ModSemL.prog.
+    unfold ModSemL.prog at 4.
+    unfold ModSemL.prog at 2.
+    Local Opaque ModSemL.prog.
+    ss. steps.
+    (* Opaque ModSemL.initial_r_state. *)
+    (* Opaque ModSemL.initial_p_state. *)
+    fold ms_src. fold ms_mid.
+    set (rs_src0 := initial_r_state ms_src) in *.
+    set (rs_tgt0 := initial_r_state ms_mid) in *.
+    assert(exists mrs_src0 hd_src tl_src, rs_src0 = (mrs_src0, hd_src :: tl_src)).
+    { esplits. refl. }
+    assert(exists mrs_tgt0 hd_tgt tl_tgt, rs_tgt0 = (mrs_tgt0, hd_tgt :: tl_tgt)).
+    { esplits. refl. }
+    des. clearbody rs_src0 rs_tgt0. subst.
+    unfold unwrapU at 1. des_ifs; cycle 1.
+    { steps. }
+    unfold unwrapU. des_ifs; cycle 1.
+    { admit "unwrapN!!!!!!!!!!". }
+
+
+    unfold ms_mid, mds_mid, SMod.to_mid in Heq0. rewrite SMod.transl_fnsems in Heq0.
+    unfold SMod.load_fnsems in Heq0. apply find_some in Heq0. des; ss. des_sumbool; subst.
+    rewrite in_flat_map in Heq0. des; ss. rewrite in_flat_map in Heq2. des; ss. des_ifs. ss; des; ss; clarify. ss. subst.
+    rename Heq2 into INF. rename Heq0 into IN.
+    rename x into md0. fold sk in INF. fold sk in INF.
+
+    unfold ms_src, mds_src, SMod.to_src in Heq. rewrite SMod.transl_fnsems in Heq.
+    unfold SMod.load_fnsems in Heq. apply find_some in Heq. des; ss. destruct p; ss. des_sumbool; subst.
+    rewrite in_flat_map in Heq. des; ss. rewrite in_flat_map in Heq0. des; ss. des_ifs. ss; des; ss; clarify.
+    rename Heq0 into INF0. rename Heq into IN0.
+    rename x into md1. fold sk in INF0. fold sk in INF0.
+
+    assert(md0 = md1); subst.
+    { admit "ez - uniqueness". }
+    assert(f = f0).
+    { admit "ez - uniqueness". }
+    subst.
+    fold ms_src. fold ms_mid. fold p_src. fold p_mid.
+
+    steps.
+
+    match goal with
+    | [ |- gpaco5 _ _ _ _ _ _ _ ?i_src _ ] => remember i_src as tmp
+    end.
+    replace (([]: list val)↑) with (Any.pair ord_top↑ ([]: list val)↑) by admit "TODO".
+    subst tmp.
+
+    guclo ordC_spec. econs.
+    { eapply OrdArith.add_base_l. }
+    guclo bindC_spec.
+    econs.
+    - hexploit adequacy_type_aux; cycle 1.
+      { intro T. gfinal. right. instantiate (3:=ord_top) in T. ss. eapply T. }
+      ss. unfold ms_src, ms_mid. unfold initial_p_state.
+      apply func_ext. intro mn. unfold mds_src, mds_mid, SMod.to_src, SMod.to_mid.
+      rewrite ! SMod.transl_initial_mrs. ss.
+    - ii. rr in SIM. des_ifs. des; ss. subst. r in SIM. des_ifs. steps.
+  Unshelve.
+    all: ss.
+    all: try (by exact Ord.O).
+    all: try (by econs; et).
+  Qed.
+
+End CANCEL.
+
+Require Import Coqlib.
+Require Import Universe.
+Require Import STS.
+Require Import Behavior.
+Require Import ModSem.
+Import ModSemL.
+Require Import Skeleton.
+Require Import PCM.
+Require Import Any.
+Require Import HoareDef.
+Require Import SimSTS.
+Require Import SimGlobal.
+Require Import HoareDef.
+From Ordinal Require Import Ordinal Arithmetic.
+
+Set Implicit Arguments.
+
+
+
+
+
+
+
+
+
+
+
+
+
+
+
+
 Inductive _simg_safe (simg: forall R (RR: R -> R -> Prop), Ord.t -> (itree eventE R) -> (itree eventE R) -> Prop)
           {R} (RR: R -> R -> Prop) (i0: Ord.t): (itree eventE R) -> (itree eventE R) -> Prop :=
 | simg_safe_ret
